@prefix cs: <http://pid.geoscience.gov.au/def/Method> .
@prefix dcterms: <http://purl.org/dc/terms/> .
@prefix rdfs: <http://www.w3.org/2000/01/rdf-schema#> .
@prefix sdo: <https://schema.org/> .
@prefix skos: <http://www.w3.org/2004/02/skos/core#> .
@prefix xsd: <http://www.w3.org/2001/XMLSchema#> .

<http://pid.geoscience.gov.au/def/Method/AAS> a skos:Concept ;
    rdfs:isDefinedBy cs: ;
    skos:altLabel "AAS"@en ;
    skos:definition "Atomic absorption spectrophotometry (AAS) is an analytical technique used to measure a wide range of elements in materials such as metals, pottery and glass. Although it is a destructive technique, th"@en ;
    skos:inScheme cs: ;
    skos:prefLabel "Atomic Absorption Spectroscopy"@en ;
    skos:scopeNote "Atomic absorption spectrophotometry (AAS) is an analytical technique used to measure a wide range of elements in materials such as metals, pottery and glass. Although it is a destructive technique, the sample size needed is very small (typically about 10 milligrams - i.e. one hundredth of a gram) and its removal causes little damage. The sample is accurately weighed and then dissolved, often using strong acids. The resulting solution is sprayed into the flame of the instrument and atomised (see schematic diagram). Light of a suitable wavelength for a particular element is shone through the flame, and some of this light is absorbed by the atoms of the sample. The amount of light absorbed is proportional to the concentration of the element in the solution, and hence in the original object. Measurements are made separately for each element of interest in turn to achieve a complete analysis of an object, and thus the technique is relatively slow to use. However, it is very sensitive and it can measure trace elements down to the part per million level, as well as being able to measure elements present in minor and major amounts."@en ;
    skos:topConceptOf cs: .

<http://pid.geoscience.gov.au/def/Method/AC> a skos:Concept ;
    rdfs:isDefinedBy cs: ;
    skos:altLabel "AC"@en ;
    skos:definition "Acid Digestion is a process of preparing analytical samples for analysis. http://en.wikipedia.org/wiki/Acid_digestion"@en ;
    skos:inScheme cs: ;
    skos:prefLabel "Acid digestion"@en ;
    skos:topConceptOf cs: .

<http://pid.geoscience.gov.au/def/Method/ADCP> a skos:Concept ;
    rdfs:isDefinedBy cs: ;
    skos:altLabel "ADCP"@en ;
    skos:definition "Measures the speed and direction across an entire water column. An ADCP can measure current speed not just at the bottom, but also at equal intervals all the way up to the surface.  The ADCP measures "@en ;
    skos:inScheme cs: ;
    skos:prefLabel "Acoustic Doppler Current Profiler"@en ;
    skos:scopeNote "Measures the speed and direction across an entire water column. An ADCP can measure current speed not just at the bottom, but also at equal intervals all the way up to the surface.  The ADCP measures water currents with sound, using a principle of sound waves called the Doppler effect. The ADCP works by transmitting \"pings\" of sound at a constant frequency into the water. As the sound waves travel, they ricochet off particles suspended in the moving water, and reflect back to the instrument. The difference in frequency between the waves the profiler sends out and the waves it receives is called the Doppler shift. The instrument uses this shift to calculate how fast the particle and the water around it are moving. www.whoi.edu/science/instruments/adcpv2.htm(.) www.nortekusa.com/prin-dop.html(.) www.sontek.com/princop/adp/adppo.htm(.) www.rdinstruments.com/products.html(.)"@en ;
    skos:topConceptOf cs: .

<http://pid.geoscience.gov.au/def/Method/AMS> a skos:Concept ;
    rdfs:isDefinedBy cs: ;
    skos:altLabel "AMS"@en ;
    skos:definition "The method suppresses molecular isobars completely and in many cases can separate atomic isobars (e.g. 14N from 14C) also. This makes possible the detection of naturally occurring, long-lived radio-is"@en ;
    skos:inScheme cs: ;
    skos:prefLabel "Accelerator mass spectrometry"@en ;
    skos:scopeNote "The method suppresses molecular isobars completely and in many cases can separate atomic isobars (e.g. 14N from 14C) also. This makes possible the detection of naturally occurring, long-lived radio-isotopes such as 10Be, 36Cl, 26Al and 14C. AMS can outperform the competing technique of decay counting for all isotopes where the half-life is long enough. http://en.wikipedia.org/wiki/Accelerator_mass_spectrometry"@en ;
    skos:topConceptOf cs: .

<http://pid.geoscience.gov.au/def/Method/APM> a skos:Concept ;
    rdfs:isDefinedBy cs: ;
    skos:altLabel "APM"@en ;
    skos:definition "Reaction of alkaline phenol and hypochlorite with ammonia to form indophenol blue which is measured photometrically. The blue colour can be intensified with sodium nitroprusside. Detection limits are "@en ;
    skos:inScheme cs: ;
    skos:prefLabel "Automated Phenate Method"@en ;
    skos:scopeNote "Reaction of alkaline phenol and hypochlorite with ammonia to form indophenol blue which is measured photometrically. The blue colour can be intensified with sodium nitroprusside. Detection limits are 0.02 to 2.0 mg/l for photometric measurements made at 630 to 660 nm in a 15mm or 50mm tubular flow cell. Interferences may include seawater, Calcium and magnesium, colour and turbidity."@en ;
    skos:topConceptOf cs: .

<http://pid.geoscience.gov.au/def/Method/Ar_Ar> a skos:Concept ;
    rdfs:isDefinedBy cs: ;
    skos:altLabel "Ar/Ar"@en ;
    skos:definition "Ar/Ar provides isotopic ages that are used to derive thermal histories of geologic materials. Samples of any age throughout Earth''s history may be dated accurately and precisely by the Ar/Ar method, "@en ;
    skos:inScheme cs: ;
    skos:prefLabel "Argon/Argon Method"@en ;
    skos:scopeNote "Ar/Ar provides isotopic ages that are used to derive thermal histories of geologic materials. Samples of any age throughout Earth''s history may be dated accurately and precisely by the Ar/Ar method, but a practical minimum age is about 10,000 years. BP. This technique, particularly when applied to various minerals within a single sample and used in conjunction with other geochronologic techniques, can provide not only the age of formation, but also its post-formation thermal and alteration history (based on argon \"closure\" temperatures in various minerals, the technique can delineate thermal history over a range of approximately 100-550¿C). Ar/Ar provides isotopic ages ranging from 10,000 years to billions of age with 0.1-0.5% precision. http://geology.cr.usgs.gov/capabilities/gronemtrac/geochron/geochron.html"@en ;
    skos:topConceptOf cs: .

<http://pid.geoscience.gov.au/def/Method/BULK> a skos:Concept ;
    rdfs:isDefinedBy cs: ;
    skos:altLabel "BULK"@en ;
    skos:definition "Bulk correlation parameters (API gravity, elemental analysis of nickel, vanadium and sulphur) of whole-oil samples are used to differentiate between oils.  These bulk parameters are used in conjunctio"@en ;
    skos:inScheme cs: ;
    skos:prefLabel "Bulk Properties"@en ;
    skos:scopeNote "Bulk correlation parameters (API gravity, elemental analysis of nickel, vanadium and sulphur) of whole-oil samples are used to differentiate between oils.  These bulk parameters are used in conjunction with biomarker ratios and carbon and hydrogen isotopes to determine oil-to-oil correlations. Petroleum Geochemistry abd Geology, Second Edition, J. M. Hunt, 1996, page 521."@en ;
    skos:topConceptOf cs: .

<http://pid.geoscience.gov.au/def/Method/Bomb> a skos:Concept ;
    rdfs:isDefinedBy cs: ;
    skos:altLabel "Bomb"@en ;
    skos:definition "The calcium carbonate content of a sample is determined by measuring the increase in gas pressure caused by acidifying a dried sediment sample in a closed vessel. The percent carbonate is then read fr"@en ;
    skos:inScheme cs: ;
    skos:prefLabel "Carbonate bomb"@en ;
    skos:scopeNote "The calcium carbonate content of a sample is determined by measuring the increase in gas pressure caused by acidifying a dried sediment sample in a closed vessel. The percent carbonate is then read from a pressure-concentration curve constructed from standard runs. Muller, G., Gastner, M., (1971)., the \"karbonate bombe\"  a simple device for the determnation of the carbonate content in sedimnet, soils and other material. Neus Fahrb. Mineral. Monatsh., 10, 466-469."@en ;
    skos:topConceptOf cs: .

<http://pid.geoscience.gov.au/def/Method/CLSM> a skos:Concept ;
    rdfs:isDefinedBy cs: ;
    skos:altLabel "CLSM"@en ;
    skos:definition "Confocal Scanning Laser Microscopy which uses spatial filtering techniques to eliminate out-of-focus light or glare in specimens whose thickness exceeds the immediate plane of focus. "@en ;
    skos:inScheme cs: ;
    skos:prefLabel "Confocal Scanning Laser Microscopy"@en ;
    skos:topConceptOf cs: .

<http://pid.geoscience.gov.au/def/Method/COL> a skos:Concept ;
    rdfs:isDefinedBy cs: ;
    skos:altLabel "COL"@en ;
    skos:definition "Colorimetry is the science that describe colour in numbers, or provides a physical colour match using a variety of measurement instruments, depending on the desired information about the colour/s the "@en ;
    skos:inScheme cs: ;
    skos:prefLabel "Colorimetry"@en ;
    skos:scopeNote "Colorimetry is the science that describe colour in numbers, or provides a physical colour match using a variety of measurement instruments, depending on the desired information about the colour/s the customer requires. http://en.wikipedia.org/wiki/Colorimetry"@en ;
    skos:topConceptOf cs: .

<http://pid.geoscience.gov.au/def/Method/CSIA_GAS> a skos:Concept ;
    rdfs:isDefinedBy cs: ;
    skos:altLabel "CSIA_GAS"@en ;
    skos:definition "Compound Specific Isotopic Analysis is a technique where different isotopes of the same compound are separated based on minute mass differences. Depending on the type of compound being analysed, the i"@en ;
    skos:inScheme cs: ;
    skos:prefLabel "Compound Specific Isotopic Analysis for gas"@en ;
    skos:scopeNote "Compound Specific Isotopic Analysis is a technique where different isotopes of the same compound are separated based on minute mass differences. Depending on the type of compound being analysed, the ion stream is prepared through either a gas chromatagraph, an elemental analyzer or the gas bench. Compound specific isotopic analysis of gas components. http://eaps.mit.edu/geobiology/biomarkers/csia.html"@en ;
    skos:topConceptOf cs: .

<http://pid.geoscience.gov.au/def/Method/CSIA_OIL> a skos:Concept ;
    rdfs:isDefinedBy cs: ;
    skos:altLabel "CSIA_OIL"@en ;
    skos:definition "Compound Specific Isotopic Analysis is a technique where different isotopes of the same compound are separated based on minute mass differences. Depending on the type of compound being analysed, the i"@en ;
    skos:inScheme cs: ;
    skos:prefLabel "Compound Specific Isotopic Analysis for oil"@en ;
    skos:scopeNote "Compound Specific Isotopic Analysis is a technique where different isotopes of the same compound are separated based on minute mass differences. Depending on the type of compound being analysed, the ion stream is prepared through either a gas chromatagraph, an elemental analyzer or directly via dual inlet. Compound specific isotopic analysis of oil components. http://eaps.mit.edu/geobiology/biomarkers/csia.html"@en ;
    skos:topConceptOf cs: .

<http://pid.geoscience.gov.au/def/Method/Calculate> a skos:Concept ;
    rdfs:isDefinedBy cs: ;
    skos:altLabel "Calculate"@en ;
    skos:definition "Method to measure Loss on Ignition. Calculated using analytical results i.e. 100 - sum of the oxides."@en ;
    skos:inScheme cs: ;
    skos:prefLabel "Calculate"@en ;
    skos:topConceptOf cs: .

<http://pid.geoscience.gov.au/def/Method/Chaix_Meca> a skos:Concept ;
    rdfs:isDefinedBy cs: ;
    skos:altLabel "Chaix Meca"@en ;
    skos:definition "Microthermometry using Chaix Meca stage (-180 to +600?C). Equipment used to study melt and fluid inclusions. The data contributes to AGSO''s ore deposit studies."@en ;
    skos:inScheme cs: ;
    skos:prefLabel "Microthermometry-Chaix Meca stage"@en ;
    skos:topConceptOf cs: .

<http://pid.geoscience.gov.au/def/Method/Chart_depth> a skos:Concept ;
    rdfs:isDefinedBy cs: ;
    skos:altLabel "Chart depth"@en ;
    skos:definition "Water depth as noted on Admiralty charts."@en ;
    skos:inScheme cs: ;
    skos:prefLabel "Chart depth"@en ;
    skos:topConceptOf cs: .

<http://pid.geoscience.gov.au/def/Method/DIC> a skos:Concept ;
    rdfs:isDefinedBy cs: ;
    skos:altLabel "DIC"@en ;
    skos:definition "A water sample is combined with a strong acid reagent.  The CO2 produced is measured by an infra-red detector.  High precision and small volume capability."@en ;
    skos:inScheme cs: ;
    skos:prefLabel "Dissolved inorganic carbon analyser"@en ;
    skos:topConceptOf cs: .

<http://pid.geoscience.gov.au/def/Method/Derivation> a skos:Concept ;
    rdfs:isDefinedBy cs: ;
    skos:altLabel "Derivation"@en ;
    skos:definition "Determination of a parameter by calculation rather than direct analysis.  For example, dissolved organic nitrogen in a water sample  is determined by the difference between the analytically determined"@en ;
    skos:inScheme cs: ;
    skos:prefLabel "Derivation"@en ;
    skos:scopeNote "Determination of a parameter by calculation rather than direct analysis.  For example, dissolved organic nitrogen in a water sample  is determined by the difference between the analytically determined values of total nitrogen and the inorganic components (NH4, NO3, NO2)"@en ;
    skos:topConceptOf cs: .

<http://pid.geoscience.gov.au/def/Method/Digestion> a skos:Concept ;
    rdfs:isDefinedBy cs: ;
    skos:altLabel "Digestion"@en ;
    skos:definition "A process of preparing sediment and water samples using chemicals and/or high temperature and pressure  to convert components of interest to an appropriate form for analysis.  The analytical finish va"@en ;
    skos:inScheme cs: ;
    skos:prefLabel "Digestion"@en ;
    skos:scopeNote "A process of preparing sediment and water samples using chemicals and/or high temperature and pressure  to convert components of interest to an appropriate form for analysis.  The analytical finish varies depending on requirement  for example ICP-OES, ICP-MS or colorimetry"@en ;
    skos:topConceptOf cs: .

<http://pid.geoscience.gov.au/def/Method/ELEMENTS> a skos:Concept ;
    rdfs:isDefinedBy cs: ;
    skos:altLabel "ELEMENTS"@en ;
    skos:definition "Elemental analysis is an experiment that determines the amount (typically a weight percent) of an element in a compound. Just as there are many different elements, there are many different experiments"@en ;
    skos:inScheme cs: ;
    skos:prefLabel "ELEMENTS"@en ;
    skos:scopeNote "Elemental analysis is an experiment that determines the amount (typically a weight percent) of an element in a compound. Just as there are many different elements, there are many different experiments for determining elemental composition. The most common type of elemental analysis is for carbon, hydrogen, and nitrogen (CHN analysis). This type of analysis is especially useful for organic compounds (compounds containing carbon-carbon bonds). http://www.chm.davidson.edu/ChemistryApplets/stoichiometry/CH.html"@en ;
    skos:topConceptOf cs: .

<http://pid.geoscience.gov.au/def/Method/EM> a skos:Concept ;
    rdfs:isDefinedBy cs: ;
    skos:altLabel "EM"@en ;
    skos:definition "One of the most commonly used methods in which an electrode is inserted into a sample, and a small current or voltage is produced,     electronically amplified and read on a meter scale. Typical tests"@en ;
    skos:inScheme cs: ;
    skos:prefLabel "Electrometric Method"@en ;
    skos:scopeNote "One of the most commonly used methods in which an electrode is inserted into a sample, and a small current or voltage is produced,     electronically amplified and read on a meter scale. Typical tests include pH and conductivity, but a variety of parameters can also be measured using ion specific electrodes (ISE) including Calcium, Nitrates, Chlorine, etc."@en ;
    skos:topConceptOf cs: .

<http://pid.geoscience.gov.au/def/Method/EOM> a skos:Concept ;
    rdfs:isDefinedBy cs: ;
    skos:altLabel "EOM"@en ;
    skos:definition "Source Rock extraction: EOM (extractable organic matter) involves pulverizing about 50 grams of rock to fine particle size, extracting the hydrocarbons with a solvent such as  dichloromethane, evapora"@en ;
    skos:inScheme cs: ;
    skos:prefLabel "Extractable Organic Matter"@en ;
    skos:scopeNote "Source Rock extraction: EOM (extractable organic matter) involves pulverizing about 50 grams of rock to fine particle size, extracting the hydrocarbons with a solvent such as  dichloromethane, evaporating the solvent, seperating the residual extract by means of colum chromotography, and analyzing the fraction by means of gas chromotography mass spectrometry. Petroleum Geochemistry abd Geology, Second Edition, J. M. Hunt, 1996, page 380."@en ;
    skos:topConceptOf cs: .

<http://pid.geoscience.gov.au/def/Method/EOS> a skos:Concept ;
    rdfs:isDefinedBy cs: ;
    skos:altLabel "EOS"@en ;
    skos:definition "Equation of State Determination that, for example, relates the thermodynamic variables of pressure, temperature, volume and number of atoms to one another. An equation of state is a formula describing"@en ;
    skos:inScheme cs: ;
    skos:prefLabel "Equation of State Determination"@en ;
    skos:scopeNote "Equation of State Determination that, for example, relates the thermodynamic variables of pressure, temperature, volume and number of atoms to one another. An equation of state is a formula describing the interconnection between various macroscopically measurable properties of a system."@en ;
    skos:topConceptOf cs: .

<http://pid.geoscience.gov.au/def/Method/ESR> a skos:Concept ;
    rdfs:isDefinedBy cs: ;
    skos:altLabel "ESR"@en ;
    skos:definition "Electron spin resonance has been used as an investigative tool for the study of radicals formed in solid materials, since the radicals typically produce an unpaired spin on the molecule from which an "@en ;
    skos:inScheme cs: ;
    skos:prefLabel "Electron Spin Resonance"@en ;
    skos:scopeNote "Electron spin resonance has been used as an investigative tool for the study of radicals formed in solid materials, since the radicals typically produce an unpaired spin on the molecule from which an electron is removed. http://hyperphysics.phy-astr.gsu.edu/hbase/molecule/esr.html"@en ;
    skos:topConceptOf cs: .

<http://pid.geoscience.gov.au/def/Method/Echo> a skos:Concept ;
    rdfs:isDefinedBy cs: ;
    skos:altLabel "Echo"@en ;
    skos:definition "An echo sounder sends high frequency sound waves through the water down to the sea floor. Sound waves bounce off solid objects, such as the ocean floor. The echo sounder measures precisely how long it"@en ;
    skos:inScheme cs: ;
    skos:prefLabel "Ship echo sounder"@en ;
    skos:scopeNote "An echo sounder sends high frequency sound waves through the water down to the sea floor. Sound waves bounce off solid objects, such as the ocean floor. The echo sounder measures precisely how long it takes for the sound waves to be returned to the surface and determines the depth based on the rate of return."@en ;
    skos:topConceptOf cs: .

<http://pid.geoscience.gov.au/def/Method/FILA> a skos:Concept ;
    rdfs:isDefinedBy cs: ;
    skos:altLabel "FILA"@en ;
    skos:definition "Equipment used for bulk leachate analysis of fluid inclusions. The small amount of fluid produced can be analysed by inductively-copuled plasma mass spectrometry (ICP MS)."@en ;
    skos:inScheme cs: ;
    skos:prefLabel "Fluid Inclusion Leachate Analysis"@en ;
    skos:topConceptOf cs: .

<http://pid.geoscience.gov.au/def/Method/Fluorometry> a skos:Concept ;
    rdfs:isDefinedBy cs: ;
    skos:altLabel "Fluorometry"@en ;
    skos:definition "Fluorometry or fluorescence spectroscopy  is a type of electromagnetic spectroscopy which analyzes fluorescence from a sample. It involves using a beam of light, usually ultraviolet light, that excite"@en ;
    skos:inScheme cs: ;
    skos:prefLabel "Fluorometer"@en ;
    skos:scopeNote "Fluorometry or fluorescence spectroscopy  is a type of electromagnetic spectroscopy which analyzes fluorescence from a sample. It involves using a beam of light, usually ultraviolet light, that excites the electrons in molecules of certain compounds and causes them to emit light of a lower energy, typically visible light."@en ;
    skos:topConceptOf cs: .

<http://pid.geoscience.gov.au/def/Method/GAS> a skos:Concept ;
    rdfs:isDefinedBy cs: ;
    skos:altLabel "GAS"@en ;
    skos:definition "Gas analysis of natural gas; the gaseous phase of petroleum. Typically a reservoir gas contains between 70 to 100 % methane (C1), 1 to 10 % ethane (C2) and lower percentages of higher hydrocarbons thr"@en ;
    skos:inScheme cs: ;
    skos:prefLabel "Gas analyses"@en ;
    skos:scopeNote "Gas analysis of natural gas; the gaseous phase of petroleum. Typically a reservoir gas contains between 70 to 100 % methane (C1), 1 to 10 % ethane (C2) and lower percentages of higher hydrocarbons through hexanes (C3-C6) and possibly traces up to nonanes (C9). Petroleum Geochemistry abd Geology, Second Edition, J. M. Hunt, 1996, page 185."@en ;
    skos:topConceptOf cs: .

<http://pid.geoscience.gov.au/def/Method/GC> a skos:Concept ;
    rdfs:isDefinedBy cs: ;
    skos:altLabel "GC"@en ;
    skos:definition "Gas chromatography is the main technique used to separate the individual components of very complex mixtures. Gas chromatography is a chromatographic technique that can be used to separate volatile or"@en ;
    skos:inScheme cs: ;
    skos:prefLabel "Gas Chromatography"@en ;
    skos:scopeNote "Gas chromatography is the main technique used to separate the individual components of very complex mixtures. Gas chromatography is a chromatographic technique that can be used to separate volatile organic compounds. A gas chromatograph consists of a flowing mobile phase, an injection port, a separation column containing the stationary phase, and a detector. The organic compounds are separated due to differences in their partitioning behavior between the mobile gas phase and the stationary phase in the column. http://elchem.kaist.ac.kr/vt/chem-ed/sep/gc/gc.htm"@en ;
    skos:topConceptOf cs: .

<http://pid.geoscience.gov.au/def/Method/GCMS_ARO_FS> a skos:Concept ;
    rdfs:isDefinedBy cs: ;
    skos:altLabel "GCMS_ARO_FS"@en ;
    skos:definition "Computerized gas chromatography - mass spectrometry (GCMS) is the principal method used to detect and identify compounds by exploiting the mass variations of different compounds. Full scan method used"@en ;
    skos:inScheme cs: ;
    skos:prefLabel "GCMS, full scan method, aromatic hydrocarbons"@en ;
    skos:scopeNote "Computerized gas chromatography - mass spectrometry (GCMS) is the principal method used to detect and identify compounds by exploiting the mass variations of different compounds. Full scan method used to detect aromatic hydrocarbon compounds. http://eaps.mit.edu/geobiology/biomarkers/gcms.html"@en ;
    skos:topConceptOf cs: .

<http://pid.geoscience.gov.au/def/Method/GCMS_ARO_MRM> a skos:Concept ;
    rdfs:isDefinedBy cs: ;
    skos:altLabel "GCMS_ARO_MRM"@en ;
    skos:definition "Computerized gas chromatography - mass spectrometry (GCMS) is the principal method used to detect and identify compounds by exploiting the mass variations of different compounds. Metastable reaction m"@en ;
    skos:inScheme cs: ;
    skos:prefLabel "GCMS, metastable reaction monitoring mode, aromatic hydrocarbons"@en ;
    skos:scopeNote "Computerized gas chromatography - mass spectrometry (GCMS) is the principal method used to detect and identify compounds by exploiting the mass variations of different compounds. Metastable reaction monitoring mode used to detect aromatic hydrocarbon compounds. http://eaps.mit.edu/geobiology/biomarkers/gcms.html"@en ;
    skos:topConceptOf cs: .

<http://pid.geoscience.gov.au/def/Method/GCMS_ARO_SIR> a skos:Concept ;
    rdfs:isDefinedBy cs: ;
    skos:altLabel "GCMS_ARO_SIR"@en ;
    skos:definition "Computerized gas chromatography - mass spectrometry (GCMS) is the principal method used to detect and identify compounds by exploiting the mass variations of different compounds. Single ion reaction m"@en ;
    skos:inScheme cs: ;
    skos:prefLabel "GCMS, single ion reaction mode, aromatic hydrocarbons"@en ;
    skos:scopeNote "Computerized gas chromatography - mass spectrometry (GCMS) is the principal method used to detect and identify compounds by exploiting the mass variations of different compounds. Single ion reaction mode used to detect aromatic hydrocarbon compounds. http://eaps.mit.edu/geobiology/biomarkers/gcms.html"@en ;
    skos:topConceptOf cs: .

<http://pid.geoscience.gov.au/def/Method/GCMS_SAT_FS> a skos:Concept ;
    rdfs:isDefinedBy cs: ;
    skos:altLabel "GCMS_SAT_FS"@en ;
    skos:definition "Computerized gas chromatography - mass spectrometry (GCMS) is the principal method used to detect and identify compounds by exploiting the mass variations of different compounds. Full scan method used"@en ;
    skos:inScheme cs: ;
    skos:prefLabel "GCMS, full scan method, saturated hydrocarbons"@en ;
    skos:scopeNote "Computerized gas chromatography - mass spectrometry (GCMS) is the principal method used to detect and identify compounds by exploiting the mass variations of different compounds. Full scan method used to detect saturated hydrocarbon compounds. http://eaps.mit.edu/geobiology/biomarkers/gcms.html"@en ;
    skos:topConceptOf cs: .

<http://pid.geoscience.gov.au/def/Method/GCMS_SAT_MRM> a skos:Concept ;
    rdfs:isDefinedBy cs: ;
    skos:altLabel "GCMS_SAT_MRM"@en ;
    skos:definition "Computerized gas chromatography - mass spectrometry (GCMS) is the principal method used to detect and identify compounds by exploiting the mass variations of different compounds. Metastable reaction m"@en ;
    skos:inScheme cs: ;
    skos:prefLabel "GCMS, metastable reaction monitoring mode, saturated hydrocarbons"@en ;
    skos:scopeNote "Computerized gas chromatography - mass spectrometry (GCMS) is the principal method used to detect and identify compounds by exploiting the mass variations of different compounds. Metastable reaction monitoring mode used to detect saturated hydrocarbon compounds. http://eaps.mit.edu/geobiology/biomarkers/gcms.html"@en ;
    skos:topConceptOf cs: .

<http://pid.geoscience.gov.au/def/Method/GCMS_SAT_SIR> a skos:Concept ;
    rdfs:isDefinedBy cs: ;
    skos:altLabel "GCMS_SAT_SIR"@en ;
    skos:definition "Computerized gas chromatography - mass spectrometry (GCMS) is the principal method used to detect and identify compounds by exploiting the mass variations of different compounds. Single ion reaction m"@en ;
    skos:inScheme cs: ;
    skos:prefLabel "GCMS, single ion reaction mode, saturated hydrocarbons"@en ;
    skos:scopeNote "Computerized gas chromatography - mass spectrometry (GCMS) is the principal method used to detect and identify compounds by exploiting the mass variations of different compounds. Single ion reaction mode used to detect saturated hydrocarbon coumpounds. http://eaps.mit.edu/geobiology/biomarkers/gcms.html"@en ;
    skos:topConceptOf cs: .

<http://pid.geoscience.gov.au/def/Method/GRS> a skos:Concept ;
    rdfs:isDefinedBy cs: ;
    skos:altLabel "GRS"@en ;
    skos:definition "Gamma ray spectrometers measure radioactive materials which emit gamma rays and are able to discriminate between radio-elements which occur naturally such as Potassium, Uranium and Thorium elements.  "@en ;
    skos:inScheme cs: ;
    skos:prefLabel "Gamma Ray Spectrometery"@en ;
    skos:scopeNote "Gamma ray spectrometers measure radioactive materials which emit gamma rays and are able to discriminate between radio-elements which occur naturally such as Potassium, Uranium and Thorium elements.  These elements are the only radioisotopes that produce gamma rays of sufficient energy and intensity to be measured at airborne survey heights. This method is applicable to ground surveys and borehole logging.  The decay of radioisotopes and their daughters can be accompanied by gamma ray emissions.  Gamma ray spectrometers record gamma rays in counts per second (cps) or counts per minute (cpm).  The fully corrected count rates can be converted to mean ground level abundances of the radioelements.  The ground concentrations of count rates in the total count, potassium, uranium and thorium channels are given in nanograys per hour (NG/h), percent (%), parts per million (ppm) and parts per million (ppm) respectively."@en ;
    skos:topConceptOf cs: .

<http://pid.geoscience.gov.au/def/Method/Gravimetry> a skos:Concept ;
    rdfs:isDefinedBy cs: ;
    skos:altLabel "Gravimetry"@en ;
    skos:definition "All Gravimetric analyses rely on some final determination of weight as a means of quantifying an analyte. Since weight can be measured with greater accuracy than almost any other fundamental property,"@en ;
    skos:inScheme cs: ;
    skos:prefLabel "Gravimetric Method"@en ;
    skos:scopeNote "All Gravimetric analyses rely on some final determination of weight as a means of quantifying an analyte. Since weight can be measured with greater accuracy than almost any other fundamental property, gravimetric analysis is potentially one of the most accurate classes of analytical methods available. These methods are among the oldest of analytical techniques, and they may be lengthy and tedious. Samples may have to be extensively treated to remove interfering substances. As a result, only a very few gravimetric methods are currently used in environmental analysis. There are four fundamental types of gravimetric analysis: physical gravimetry, thermogravimetry, precipitative gravimetric analysis, and electrodeposition. These differ in the preparation of the sample before weighing of the analyte. Physical gravimetry is the most common type used in environmental engineering. It involves the physical separation and classification of matter in environmental samples based on volatility and particle size (e.g., total suspended solids). With thermogravimetry, samples are heated and changes in sample mass are recorded. Volatile solids analysis is an important example of this type of gravimetric analysis. As the name implies, precipitative gravimetry relies on the chemical precipitation of an analyte. Its most important application in the environmental field is with the analysis of sulfite. Electrodeposition involves the electrochemical reduction of metal ions at a cathode, and simultaneous deposition of the ions on the cathode."@en ;
    skos:topConceptOf cs: .

<http://pid.geoscience.gov.au/def/Method/H20> a skos:Concept ;
    rdfs:isDefinedBy cs: ;
    skos:altLabel "H20"@en ;
    skos:definition "Analysis of formation water broken down to the trace elements and nutrients such as nitrogen, phosphorus, halogens (chloride and fluoride ions), alkali metals (sodium and potassium ions), calcium and "@en ;
    skos:inScheme cs: ;
    skos:prefLabel "Water Analysis"@en ;
    skos:scopeNote "Analysis of formation water broken down to the trace elements and nutrients such as nitrogen, phosphorus, halogens (chloride and fluoride ions), alkali metals (sodium and potassium ions), calcium and magnesium ions to determine water quality. Also describes physical properties including resistivity, pH, conductivity etc."@en ;
    skos:topConceptOf cs: .

<http://pid.geoscience.gov.au/def/Method/ICA> a skos:Concept ;
    rdfs:isDefinedBy cs: ;
    skos:altLabel "ICA"@en ;
    skos:definition "Chromatography relies on the different partitioning behaviour of molecules between a mobile phase (eluent) and stationary phase (column packed with resin). Ion chromatography uses ion exchange resins "@en ;
    skos:inScheme cs: ;
    skos:prefLabel "Ion Chromatographic Analysis"@en ;
    skos:scopeNote "Chromatography relies on the different partitioning behaviour of molecules between a mobile phase (eluent) and stationary phase (column packed with resin). Ion chromatography uses ion exchange resins to separate ions based on their interactions with the resin. Each element is identified based on its rate of elution from the column and the concentration is proportional to e.g. electrical conductivity of the eluted solution."@en ;
    skos:topConceptOf cs: .

<http://pid.geoscience.gov.au/def/Method/ICP-MS> a skos:Concept ;
    rdfs:isDefinedBy cs: ;
    skos:altLabel "ICP-MS"@en ;
    skos:definition "ICPMS: Instrumental Plasma Mass Spectrometry: A sample is vapourised into a plasma gas and ions are accelerated down a flight tube of a mass spectrometer between magnets. Elements are separated by the"@en ;
    skos:inScheme cs: ;
    skos:prefLabel "Inductively Coupled Plasma Mass Spectrometry"@en ;
    skos:scopeNote "ICPMS: Instrumental Plasma Mass Spectrometry: A sample is vapourised into a plasma gas and ions are accelerated down a flight tube of a mass spectrometer between magnets. Elements are separated by their difference in mass. Can analyse a wide range of elements to as low as 0.01 ppm."@en ;
    skos:topConceptOf cs: .

<http://pid.geoscience.gov.au/def/Method/ICP-OES> a skos:Concept ;
    rdfs:isDefinedBy cs: ;
    skos:altLabel "ICP-OES"@en ;
    skos:definition "ICP-OES is a multi-element simultaneous technique for elemental analysis of cations (e.g. Na, K, Ca, Mg, Fe, Al, Mn etc.), sulphur, phosphorous and silicon. The high temperature of the plasma vaporise"@en ;
    skos:inScheme cs: ;
    skos:prefLabel "Inductively Coupled Plasma Optical Emission Spectrometer"@en ;
    skos:scopeNote "ICP-OES is a multi-element simultaneous technique for elemental analysis of cations (e.g. Na, K, Ca, Mg, Fe, Al, Mn etc.), sulphur, phosphorous and silicon. The high temperature of the plasma vaporises the aerosol and excites the atoms to high energy levels.  On returning to their ground state the spectrum of wavelengths emitted can be used to identify the element that it originated from."@en ;
    skos:topConceptOf cs: .

<http://pid.geoscience.gov.au/def/Method/INAA> a skos:Concept ;
    rdfs:isDefinedBy cs: ;
    skos:altLabel "INAA"@en ;
    skos:definition "Neutron activation analysis (NAA) is a techniques used for qualitative and quantitative elemental analysis of multiple major, minor, and trace elements in samples from almost every conceivable field o"@en ;
    skos:inScheme cs: ;
    skos:prefLabel "Instrumental Neutron Activation Analysis"@en ;
    skos:scopeNote "Neutron activation analysis (NAA) is a techniques used for qualitative and quantitative elemental analysis of multiple major, minor, and trace elements in samples from almost every conceivable field of scientific or technical interest. For many elements, NAA offers sensitivities that are superior to those possible by any other technique."@en ;
    skos:topConceptOf cs: .

<http://pid.geoscience.gov.au/def/Method/IRMS> a skos:Concept ;
    rdfs:isDefinedBy cs: ;
    skos:altLabel "IRMS"@en ;
    skos:definition "Measures the relative abundances of stable isotopes in a sample by measuring isotopic variations arising from mass-dependent isotopic fractionation in natural systems. Mass spectrometry distinguishes "@en ;
    skos:inScheme cs: ;
    skos:prefLabel "Isotope Ratio Mass Spectrometer"@en ;
    skos:scopeNote "Measures the relative abundances of stable isotopes in a sample by measuring isotopic variations arising from mass-dependent isotopic fractionation in natural systems. Mass spectrometry distinguishes elements based on a mass to charge ratio."@en ;
    skos:topConceptOf cs: .

<http://pid.geoscience.gov.au/def/Method/ISOTOPES> a skos:Concept ;
    rdfs:isDefinedBy cs: ;
    skos:altLabel "ISOTOPES"@en ;
    skos:definition "Isotopic composition of organic components"@en ;
    skos:inScheme cs: ;
    skos:prefLabel "Isotopic composition of organic components"@en ;
    skos:topConceptOf cs: .

<http://pid.geoscience.gov.au/def/Method/ISOTOPES_IN> a skos:Concept ;
    rdfs:isDefinedBy cs: ;
    skos:altLabel "ISOTOPES_IN"@en ;
    skos:definition "Isotopic composition of inorganic components"@en ;
    skos:inScheme cs: ;
    skos:prefLabel "Isotopic composition of inorganic components"@en ;
    skos:topConceptOf cs: .

<http://pid.geoscience.gov.au/def/Method/KINETICS> a skos:Concept ;
    rdfs:isDefinedBy cs: ;
    skos:altLabel "KINETICS"@en ;
    skos:definition "Chemical kinetics is a scientific discipline dedicated to the study of the rates of chemical reactions. How fast is a reaction proceeding in time, and what is affecting the rate. http://www.corrosion-"@en ;
    skos:inScheme cs: ;
    skos:prefLabel "Chemical kinetics for hydrocarbon generation"@en ;
    skos:scopeNote "Chemical kinetics is a scientific discipline dedicated to the study of the rates of chemical reactions. How fast is a reaction proceeding in time, and what is affecting the rate. http://www.corrosion-doctors.org/Dictionary/Dictionary-K.htm"@en ;
    skos:topConceptOf cs: .

<http://pid.geoscience.gov.au/def/Method/K_Ar> a skos:Concept ;
    rdfs:isDefinedBy cs: ;
    skos:altLabel "K/Ar"@en ;
    skos:definition "The Potassium-Argon (K-Ar) dating method is the measurement of the accumulation of argon in a mineral. K-Ar dating measure the accumulation of argon in a substance from the decomposition of potassium."@en ;
    skos:inScheme cs: ;
    skos:prefLabel "Potassium/Argon Method"@en ;
    skos:scopeNote "The Potassium-Argon (K-Ar) dating method is the measurement of the accumulation of argon in a mineral. K-Ar dating measure the accumulation of argon in a substance from the decomposition of potassium. http://www.mnsu.edu/emuseum/archaeology/dating/dat_ka.html"@en ;
    skos:topConceptOf cs: .

<http://pid.geoscience.gov.au/def/Method/LA-ICP-MS> a skos:Concept ;
    rdfs:isDefinedBy cs: ;
    skos:altLabel "LA-ICP-MS"@en ;
    skos:definition "Laser Ablation-Inductively Coupled Plasma-Mass Spectrometry. Equipment that uses a laser to drill into a sub-surface inclusion and vaporise the inclusion contents which are then transferred in a carri"@en ;
    skos:inScheme cs: ;
    skos:prefLabel "Mass Spectrometry-Laser Ablation-Inductively Coupled Plasma"@en ;
    skos:scopeNote "Laser Ablation-Inductively Coupled Plasma-Mass Spectrometry. Equipment that uses a laser to drill into a sub-surface inclusion and vaporise the inclusion contents which are then transferred in a carrier gas to a mass spectrometer for analysis and identification."@en ;
    skos:topConceptOf cs: .

<http://pid.geoscience.gov.au/def/Method/LECO> a skos:Concept ;
    rdfs:isDefinedBy cs: ;
    skos:altLabel "LECO"@en ;
    skos:definition "The total carbon content of a sediment sample is determined by measuring the thermal conductivty of the gaseous products of pyrolysis of the sample. The analysis may also be conducted on an acidified "@en ;
    skos:inScheme cs: ;
    skos:prefLabel "LECO"@en ;
    skos:scopeNote "The total carbon content of a sediment sample is determined by measuring the thermal conductivty of the gaseous products of pyrolysis of the sample. The analysis may also be conducted on an acidified sample to determine the organic carbon content. The weight percentages of total carbon (TC), organic carbon (OC), and calcium carbonate (CaCO3) are related by the equation:  (TC - OC) * 8.33 = CaCO3. The actual file value for CaCO3 may vary from this formula by as much as 1.67 percent (0.2 * 8.33) due to an early procedural  much as 1.67 percent (0.2 * 8.33) due to an early procedural error which truncated rather than rounded the values reported for total carbon and organic carbon."@en ;
    skos:topConceptOf cs: .

<http://pid.geoscience.gov.au/def/Method/LRMP> a skos:Concept ;
    rdfs:isDefinedBy cs: ;
    skos:altLabel "LRMP"@en ;
    skos:definition "Laser Raman Microprobe. The Laser Raman Microprobe is used for the rapid identification and non-destructive analysis of solids, liquids and gases. The high spatial resolution of this instrument (down "@en ;
    skos:inScheme cs: ;
    skos:prefLabel "Laser Raman Microprobe "@en ;
    skos:scopeNote "Laser Raman Microprobe. The Laser Raman Microprobe is used for the rapid identification and non-destructive analysis of solids, liquids and gases. The high spatial resolution of this instrument (down to 1 mm) makes it p"@en ;
    skos:topConceptOf cs: .

<http://pid.geoscience.gov.au/def/Method/Laser> a skos:Concept ;
    rdfs:isDefinedBy cs: ;
    skos:altLabel "Laser"@en ;
    skos:definition "In laser diffraction particle size analysis, a representative cloud of particles passes through a broadened beam of laser light which scatters the incident light onto a Fourier lens. This lens focuses"@en ;
    skos:inScheme cs: ;
    skos:prefLabel "Laser Particle Size Analyser"@en ;
    skos:scopeNote "In laser diffraction particle size analysis, a representative cloud of particles passes through a broadened beam of laser light which scatters the incident light onto a Fourier lens. This lens focuses the scattered light onto a detector array and, using an inversion algorithm, a particle size distribution is inferred from the collected diffracted light data. Malvern Instruments Ltd, Worcestershire, UK."@en ;
    skos:topConceptOf cs: .

<http://pid.geoscience.gov.au/def/Method/Leica_1350> a skos:Concept ;
    rdfs:isDefinedBy cs: ;
    skos:altLabel "Leica 1350"@en ;
    skos:definition "Microthermometry using Leica 1350 stage (25 to 1350?C). Equipment used to study melt and fluid inclusions."@en ;
    skos:inScheme cs: ;
    skos:prefLabel "Microthermometry-Leica 1350 stage"@en ;
    skos:topConceptOf cs: .

<http://pid.geoscience.gov.au/def/Method/Lk-MDS600> a skos:Concept ;
    rdfs:isDefinedBy cs: ;
    skos:altLabel "Lk-MDS600"@en ;
    skos:definition "Microthermometry using computerised Linkam MDS 600 stage (-196 to +600C). Equipment used to study melt and fluid inclusions. "@en ;
    skos:inScheme cs: ;
    skos:prefLabel "Microthermometry-Linkam MDS 600 Stage"@en ;
    skos:topConceptOf cs: .

<http://pid.geoscience.gov.au/def/Method/Lk-THM600> a skos:Concept ;
    rdfs:isDefinedBy cs: ;
    skos:altLabel "Lk-THM600"@en ;
    skos:definition "Microthermometry using Linkam THM 600 stage (-196 to +600?C). Equipment used to study melt and fluid inclusions"@en ;
    skos:inScheme cs: ;
    skos:prefLabel "Microthermometry-Linkham THM600 stage"@en ;
    skos:topConceptOf cs: .

<http://pid.geoscience.gov.au/def/Method/Lk-TS1500> a skos:Concept ;
    rdfs:isDefinedBy cs: ;
    skos:altLabel "Lk-TS1500"@en ;
    skos:definition "Microthermometry using Linkam TS 1500 stage (25 to 1500?C). Equipment used to study melt and fluid inclusions. "@en ;
    skos:inScheme cs: ;
    skos:prefLabel "Microthermometry-Linkam TS 1500 stage"@en ;
    skos:topConceptOf cs: .

<http://pid.geoscience.gov.au/def/Method/MF> a skos:Concept ;
    rdfs:isDefinedBy cs: ;
    skos:altLabel "MF"@en ;
    skos:definition "The MF method provides a direct count of bacteria in water based on the development of colonies on the surface of the membrane filter. A water sample is filtered through the membrane which retains the"@en ;
    skos:inScheme cs: ;
    skos:prefLabel "Membrane Filter"@en ;
    skos:scopeNote "The MF method provides a direct count of bacteria in water based on the development of colonies on the surface of the membrane filter. A water sample is filtered through the membrane which retains the bacteria."@en ;
    skos:topConceptOf cs: .

<http://pid.geoscience.gov.au/def/Method/MIMS> a skos:Concept ;
    rdfs:isDefinedBy cs: ;
    skos:altLabel "MIMS"@en ;
    skos:definition "High precision measurement of dissolved gases e.g. oxygen and isotopes of nitrogen, in water samples. A semi-permeable membrane sample introduction system is coupled to a quadropole mass spectrometer."@en ;
    skos:inScheme cs: ;
    skos:prefLabel "Membrane Inlet Mass Spectrometry"@en ;
    skos:topConceptOf cs: .

<http://pid.geoscience.gov.au/def/Method/MPIP> a skos:Concept ;
    rdfs:isDefinedBy cs: ;
    skos:altLabel "MPIP"@en ;
    skos:definition "Micro-Photography and Image Processing - includes both digital and film cameras attached to microscopes and image enhancement processes performed on digital images."@en ;
    skos:inScheme cs: ;
    skos:prefLabel "Micro-Photography and Image Processing"@en ;
    skos:topConceptOf cs: .

<http://pid.geoscience.gov.au/def/Method/MacFlinCor> a skos:Concept ;
    rdfs:isDefinedBy cs: ;
    skos:altLabel "MacFlinCor"@en ;
    skos:definition "Macintosh HyperCard program. Software for the calculation of the chemical properties of fluid inclusions. Developed by Phillip Brown, University of Wisconsin."@en ;
    skos:inScheme cs: ;
    skos:prefLabel "Macintosh HyperCard program"@en ;
    skos:topConceptOf cs: .

<http://pid.geoscience.gov.au/def/Method/Microscopy> a skos:Concept ;
    rdfs:isDefinedBy cs: ;
    skos:altLabel "Microscopy"@en ;
    skos:definition "Optical Microscopic Analysis. Any observations or measurements made through a conventional optical microscope in either transmitted or reflected light."@en ;
    skos:inScheme cs: ;
    skos:prefLabel "Microscopy-Optical"@en ;
    skos:topConceptOf cs: .

<http://pid.geoscience.gov.au/def/Method/NMM> a skos:Concept ;
    rdfs:isDefinedBy cs: ;
    skos:altLabel "NMM"@en ;
    skos:definition "Nuclear Microprobe Microanalysis - includes all microfocusing instruments using atomic or subatomic particles"@en ;
    skos:inScheme cs: ;
    skos:prefLabel "Neuclear Microprobe Microanalysis"@en ;
    skos:topConceptOf cs: .

<http://pid.geoscience.gov.au/def/Method/OIL_FRACTION> a skos:Concept ;
    rdfs:isDefinedBy cs: ;
    skos:altLabel "OIL_FRACTION"@en ;
    skos:definition "Oil/condensate preparation; column chromatography and molecular sieving. Column chromatography: a mixture is separated by distributing the components between a stationary phase and a mobile phase. The"@en ;
    skos:inScheme cs: ;
    skos:prefLabel "OIL_FRACTION"@en ;
    skos:scopeNote "Oil/condensate preparation; column chromatography and molecular sieving. Column chromatography: a mixture is separated by distributing the components between a stationary phase and a mobile phase. The mixture is first placed on the stationary phase (a solid or a liquid) and then the mobile phase (a gas or a liquid) is allowed to pass through the system. The stationary phase is a powdered adsorbent which is placed in a vertical glass column. The mixture to be analysed is loaded on top of this column. The mobile phase is a solvent poured on top of the loaded column. The solvent flows down the column, causing the components of the mixture to distribute between the powdered adsorbent and the solvent, thus separating the components of the mixture so that as the solvent flows out of the bottom of the column, some components elute with early collections and other components elute with late fractions. http://orgchem.colorado.edu/hndbksupport/chrom.html"@en ;
    skos:topConceptOf cs: .

<http://pid.geoscience.gov.au/def/Method/PIXE> a skos:Concept ;
    rdfs:isDefinedBy cs: ;
    skos:altLabel "PIXE"@en ;
    skos:definition "Proton Induced X-Ray Emission (PIXE) analysis irradiates a fluid inclusion with a high energy proton beam to produce X-rays that are characteristic of the chemical elements within the inclusion."@en ;
    skos:inScheme cs: ;
    skos:prefLabel "Proton Induced X-Ray Emission"@en ;
    skos:topConceptOf cs: .

<http://pid.geoscience.gov.au/def/Method/PY_GC> a skos:Concept ;
    rdfs:isDefinedBy cs: ;
    skos:altLabel "PY_GC"@en ;
    skos:definition "Pyrolysis-Gas Chromatography: A version of reaction chromatography in which a sample is thermally decomposed to simpler fragments before entering the column of a gas chromatograph. http://www.iupac.or"@en ;
    skos:inScheme cs: ;
    skos:prefLabel "Pyrolysis-Gas Chromatography"@en ;
    skos:scopeNote "Pyrolysis-Gas Chromatography: A version of reaction chromatography in which a sample is thermally decomposed to simpler fragments before entering the column of a gas chromatograph. http://www.iupac.org/goldbook/P04962.pdf"@en ;
    skos:topConceptOf cs: .

<http://pid.geoscience.gov.au/def/Method/REFLECTANCE> a skos:Concept ;
    rdfs:isDefinedBy cs: ;
    skos:altLabel "REFLECTANCE"@en ;
    skos:definition "Petrographic analysis using reflected light microscopy determining the rank and maceral composition of a sample."@en ;
    skos:inScheme cs: ;
    skos:prefLabel "REFLECTANCE"@en ;
    skos:topConceptOf cs: .

<http://pid.geoscience.gov.au/def/Method/ROCKEVAL> a skos:Concept ;
    rdfs:isDefinedBy cs: ;
    skos:altLabel "ROCKEVAL"@en ;
    skos:definition "This method is based on a whole-rock pyrolysis technique designed to identify the type of organic matter and its maturity and to evaluate the petroleum potential of sediments (Espitali¿ et al., 1986)."@en ;
    skos:inScheme cs: ;
    skos:prefLabel "ROCKEVAL"@en ;
    skos:scopeNote "This method is based on a whole-rock pyrolysis technique designed to identify the type of organic matter and its maturity and to evaluate the petroleum potential of sediments (Espitali¿ et al., 1986). Some instruments also provide a measure of TOC. The technique involves passing a stream of helium through 100 mg of pulverized rock heated initially to 300 deg C. The temperature is then programmed to increase about 25 deg C/min, up to 55 deg C. The vapours are analyzed with a flame ionization detector (FID). S1 represents any free hydrocarbons in the rock that either were present at the time of deposition or were generated from the kerogen since deposition. Heating to 300 deg C distills free hydrocarbons from organic matter (kerogen and bitumen) in the rock. The carboxyl groups in the kerogen break off between 300 and 390 deg C, yielding CO2. Between 350 and 550 deg C, hydrocarbons are generated by cracking the kerogen until only residual, nongenrating carbon remains. Petroleum Geochemistry abd Geology, Second Edition, J. M. Hunt, 1996, page 341."@en ;
    skos:topConceptOf cs: .

<http://pid.geoscience.gov.au/def/Method/Rb_Sr> a skos:Concept ;
    rdfs:isDefinedBy cs: ;
    skos:altLabel "Rb/Sr"@en ;
    skos:definition "A geochronological method to determine emplacement ages or cooling ages of specific minerals. Rb/Sr method provides isotopic ages ranging from Precambrian (older than 570 million years) except in spec"@en ;
    skos:inScheme cs: ;
    skos:prefLabel "Rubidium/Strontium Method"@en ;
    skos:scopeNote "A geochronological method to determine emplacement ages or cooling ages of specific minerals. Rb/Sr method provides isotopic ages ranging from Precambrian (older than 570 million years) except in specific circumstances. http://geology.cr.usgs.gov/capabilities/gronemtrac/geochron/geochron.html"@en ;
    skos:topConceptOf cs: .

<http://pid.geoscience.gov.au/def/Method/Rock-colour_Chart> a skos:Concept ;
    rdfs:isDefinedBy cs: ;
    skos:altLabel "Rock-colour Chart"@en ;
    skos:definition "A standard rock  colour chart produced by the Geological Society of America in 1959 and updated in 2001"@en ;
    skos:inScheme cs: ;
    skos:prefLabel "Rock-colour Chart"@en ;
    skos:topConceptOf cs: .

<http://pid.geoscience.gov.au/def/Method/SAA> a skos:Concept ;
    rdfs:isDefinedBy cs: ;
    skos:altLabel "SAA"@en ;
    skos:definition "Surface Area Analysis entails the measurement of the external surface area of a solid(termed the adsorbent)by using a gas which is capable of being adsorbed(termed the adsorptive) using GA current ins"@en ;
    skos:inScheme cs: ;
    skos:prefLabel "Surface Area Analysis"@en ;
    skos:scopeNote "Surface Area Analysis entails the measurement of the external surface area of a solid(termed the adsorbent)by using a gas which is capable of being adsorbed(termed the adsorptive) using GA current instrument of Quantachrome Nova 2200e Surface Area & Pore Size Analyser and produce a result in m2/gm."@en ;
    skos:topConceptOf cs: .

<http://pid.geoscience.gov.au/def/Method/SEMCL> a skos:Concept ;
    rdfs:isDefinedBy cs: ;
    skos:altLabel "SEMCL"@en ;
    skos:definition "SEM-Based Cathodoluminescence Imagery produces coloured images of crystals where different shadings correspond to different chemical compositions within the crystals."@en ;
    skos:inScheme cs: ;
    skos:prefLabel "SEM-Based Cathodoluminescence Imagery"@en ;
    skos:topConceptOf cs: .

<http://pid.geoscience.gov.au/def/Method/SHRIMP> a skos:Concept ;
    rdfs:isDefinedBy cs: ;
    skos:altLabel "SHRIMP"@en ;
    skos:definition "Sensitive High Resolution Ion Microprobe technique is a method of  the dating rocks and minerals using radioactive isotopes. Using the SHRIMP, selected areas of growth on single grains of zircon, badd"@en ;
    skos:inScheme cs: ;
    skos:prefLabel "Sensitive High Resolution Ion Microprobe"@en ;
    skos:scopeNote "Sensitive High Resolution Ion Microprobe technique is a method of  the dating rocks and minerals using radioactive isotopes. Using the SHRIMP, selected areas of growth on single grains of zircon, baddeleyite, sphene, rutile and monazite can be accurately dated (to less than 100 000 years in some cases). This technique not only dates older mineral cores (what we call inherited cores), but also later magmatic and/or metamorphic overgrowths so that it unravels the entire geological history of a single mineral grain. http://www.amonline.net.au/geoscience/earth/dating.htm#shrimp"@en ;
    skos:topConceptOf cs: .

<http://pid.geoscience.gov.au/def/Method/STM> a skos:Concept ;
    rdfs:isDefinedBy cs: ;
    skos:altLabel "STM"@en ;
    skos:definition "There are two types of spectrophotometric methods: trichromatic and monochromatic. Trichromatic methods have been developed in order to determine the three types of chlorophyll (a, b, and c) in the ab"@en ;
    skos:inScheme cs: ;
    skos:prefLabel "Spectrophotometric/Trichromatic Method"@en ;
    skos:scopeNote "There are two types of spectrophotometric methods: trichromatic and monochromatic. Trichromatic methods have been developed in order to determine the three types of chlorophyll (a, b, and c) in the absence of degradation products. Absorbances must be measured at the three maximum wavelengths of the three chlorophylls, plus a blank wavelength, then a set of three equations is used to calculate the concentrations."@en ;
    skos:topConceptOf cs: .

<http://pid.geoscience.gov.au/def/Method/SYNCXRF> a skos:Concept ;
    rdfs:isDefinedBy cs: ;
    skos:altLabel "SYNCXRF"@en ;
    skos:definition "Synchotron X-ray Fluorescence spectroscopy uses an intense X-ray beam from a synchrotron to produce X-ray fluorescence from compounds within individual fluid inclusions."@en ;
    skos:inScheme cs: ;
    skos:prefLabel "Synchotron XRF"@en ;
    skos:topConceptOf cs: .

<http://pid.geoscience.gov.au/def/Method/Settling_Tube> a skos:Concept ;
    rdfs:isDefinedBy cs: ;
    skos:altLabel "Settling Tube"@en ;
    skos:definition "Settling tube Apparatus designed to determine rapidly the grain-size distribution of sand-sized sediment. The sedimentation-tube method is based on the principle of Stokes law that particles of differ"@en ;
    skos:inScheme cs: ;
    skos:prefLabel "Settling Tube Or Sedimentation Tube"@en ;
    skos:scopeNote "Settling tube Apparatus designed to determine rapidly the grain-size distribution of sand-sized sediment. The sedimentation-tube method is based on the principle of Stokes law that particles of different sizes, shapes, and densities will settle through a column of fluid at different settling velocities. Sediment is introduced into the top of the settling tube, and the time is recorded for the various sediment fractions to settle to the bottom of the tube."@en ;
    skos:topConceptOf cs: .

<http://pid.geoscience.gov.au/def/Method/Sieve> a skos:Concept ;
    rdfs:isDefinedBy cs: ;
    skos:altLabel "Sieve"@en ;
    skos:definition "Grain size analysis is used to determine the percentages of the mud, sand and gravel fractions of a sample, and then examine these fractions. This is done by splitting the sample into the separate fra"@en ;
    skos:inScheme cs: ;
    skos:prefLabel "Sieve grain size"@en ;
    skos:scopeNote "Grain size analysis is used to determine the percentages of the mud, sand and gravel fractions of a sample, and then examine these fractions. This is done by splitting the sample into the separate fractions, using a wet sieving method, and then determining the percentages of these fractions by weight.  These fractions can then be individually examined under a microscope. Generally, Udden and Wentworth Seives are used."@en ;
    skos:topConceptOf cs: .

<http://pid.geoscience.gov.au/def/Method/Sm_Nd> a skos:Concept ;
    rdfs:isDefinedBy cs: ;
    skos:altLabel "Sm/Nd"@en ;
    skos:definition "A geochronological method to determine age of crystallization/emplacement. Sm/Nd method provides isotopic ages ranging from Tertiary (last 65 million yrs) through Archean (last 3.8 billion yrs), but o"@en ;
    skos:inScheme cs: ;
    skos:prefLabel "Samarium/Neodymium Method"@en ;
    skos:scopeNote "A geochronological method to determine age of crystallization/emplacement. Sm/Nd method provides isotopic ages ranging from Tertiary (last 65 million yrs) through Archean (last 3.8 billion yrs), but of limited use in highly-metamorphic terranes. http://geology.cr.usgs.gov/capabilities/gronemtrac/geochron/geochron.html"@en ;
    skos:topConceptOf cs: .

<http://pid.geoscience.gov.au/def/Method/Sync-FTIR> a skos:Concept ;
    rdfs:isDefinedBy cs: ;
    skos:altLabel "Sync-FTIR"@en ;
    skos:definition "Syncrotron-FTIR-Microspectrometry"@en ;
    skos:inScheme cs: ;
    skos:prefLabel "Microspectrometry-Syncrotron-FTIR"@en ;
    skos:topConceptOf cs: .

<http://pid.geoscience.gov.au/def/Method/TIT> a skos:Concept ;
    rdfs:isDefinedBy cs: ;
    skos:altLabel "TIT"@en ;
    skos:definition " Titration a measured amount of a solution of unknown concentration is added to a known volume of a second solution until the reaction between them is just complete; the concentration of the unknown s"@en ;
    skos:inScheme cs: ;
    skos:prefLabel "Titration"@en ;
    skos:scopeNote " Titration a measured amount of a solution of unknown concentration is added to a known volume of a second solution until the reaction between them is just complete; the concentration of the unknown solution (the titer) can them be calculated."@en ;
    skos:topConceptOf cs: .

<http://pid.geoscience.gov.au/def/Method/Transmissometry_> a skos:Concept ;
    rdfs:isDefinedBy cs: ;
    skos:altLabel "Transmissometry "@en ;
    skos:definition "A kind of turbidity measurement in which a calibrated beam of light is projected through the water sample to a light detector over a set distance (usually less than 300mm). The loss in the intensity o"@en ;
    skos:inScheme cs: ;
    skos:prefLabel "Transmissometry"@en ;
    skos:scopeNote "A kind of turbidity measurement in which a calibrated beam of light is projected through the water sample to a light detector over a set distance (usually less than 300mm). The loss in the intensity or absorption of light is then measured and correlated to the turbidity."@en ;
    skos:topConceptOf cs: .

<http://pid.geoscience.gov.au/def/Method/Turbidimetry> a skos:Concept ;
    rdfs:isDefinedBy cs: ;
    skos:altLabel "Turbidimetry"@en ;
    skos:definition "It is an optical property that expresses the degree to which light is scattered and absorbed by molecules and particles in the sample."@en ;
    skos:inScheme cs: ;
    skos:prefLabel "Turbidimetry"@en ;
    skos:topConceptOf cs: .

<http://pid.geoscience.gov.au/def/Method/USGS_H_F> a skos:Concept ;
    rdfs:isDefinedBy cs: ;
    skos:altLabel "USGS H/F"@en ;
    skos:definition "Microthermometry using Fluidinc modified USGS gas flow stage (-180 to +700?C). Equipment used to study melt and fluid inclusions."@en ;
    skos:inScheme cs: ;
    skos:prefLabel "Microthermometry-Fluidinc modified USGS gas flow stage"@en ;
    skos:topConceptOf cs: .

<http://pid.geoscience.gov.au/def/Method/UV_VIS> a skos:Concept ;
    rdfs:isDefinedBy cs: ;
    skos:altLabel "UV/VIS"@en ;
    skos:definition "UV-VIS spectrophotometry is the measurement of the wavelength and intensity of absorption or transmission of near-ultraviolet and visible light (180 to 820 nm) by a sample. Absorption occurs when ligh"@en ;
    skos:inScheme cs: ;
    skos:prefLabel "Ultraviolet-visible spectrophotometry"@en ;
    skos:scopeNote "UV-VIS spectrophotometry is the measurement of the wavelength and intensity of absorption or transmission of near-ultraviolet and visible light (180 to 820 nm) by a sample. Absorption occurs when light is energetic enough to promote outer electrons to higher energy levels. The interaction between light absorbance and the sample is dependent on the wavelength of the light and the molecular structure of the sample. It is routinely used in the quantitative determination of solutions of transition metal ions and highly conjugated organic compounds. The Beer-Lambert law states that the absorbance of a solution is directly proportional to the solution''s concentration. Thus UV/VIS spectroscopy can be used to determine the concentration of a solution."@en ;
    skos:topConceptOf cs: .

<http://pid.geoscience.gov.au/def/Method/U_Pb_Conventional> a skos:Concept ;
    rdfs:isDefinedBy cs: ;
    skos:altLabel "U/Pb Conventional"@en ;
    skos:definition "U-Pb geochronology of zircon, baddelyite, and monazite is used for determining the age of emplacement of igneous rocks of all compositions, ranging in age from Tertiary to Early Archean. U-Pb ages of "@en ;
    skos:inScheme cs: ;
    skos:prefLabel "Uranium/Lead Conventional Method"@en ;
    skos:scopeNote "U-Pb geochronology of zircon, baddelyite, and monazite is used for determining the age of emplacement of igneous rocks of all compositions, ranging in age from Tertiary to Early Archean. U-Pb ages of metamorphic minerals, such as zircon, sphene and monazite are used to date thermal events, including terrestrial meteoritic impacts, and to determine thermochronologic histories of terranes. U-Pb ages of zircon in sediments are used to determine the provenance of the sediments. U/Pb method provides isotopic ages ranging from Archean (3.8 billion years) to early Tertiary (last 65 million years), possibly mid Teritary. http://geology.cr.usgs.gov/capabilities/gronemtrac/geochron/geochron.html"@en ;
    skos:topConceptOf cs: .

<http://pid.geoscience.gov.au/def/Method/Unknown> a skos:Concept ;
    rdfs:isDefinedBy cs: ;
    skos:altLabel "Unknown"@en ;
    skos:definition "The method of observation or measurement is unknown"@en ;
    skos:inScheme cs: ;
    skos:prefLabel "Unknown"@en ;
    skos:topConceptOf cs: .

<http://pid.geoscience.gov.au/def/Method/VGT> a skos:Concept ;
    rdfs:isDefinedBy cs: ;
    skos:altLabel "VGT"@en ;
    skos:definition "With this technique a small sample, ~0.25 g, is digested in concentrated phosphoric acid under vacuum and the pressure generated by the release of CO2 recorded on a vacuum gauge. Percent CaCO3 is calc"@en ;
    skos:inScheme cs: ;
    skos:prefLabel "Vacuum Gasometric Technique"@en ;
    skos:scopeNote "With this technique a small sample, ~0.25 g, is digested in concentrated phosphoric acid under vacuum and the pressure generated by the release of CO2 recorded on a vacuum gauge. Percent CaCO3 is calculated by relating the pressure increase in the sample to the pressure increase in reagent carbonate after correcting for temperature and pressure. http://www-odp.tamu.edu/publications/164_SR/chap_31/ch31_4.htm  http://jsedres.geoscienceworld.org/content/53/2/655.full.pdf?ck=nck"@en ;
    skos:topConceptOf cs: .

<http://pid.geoscience.gov.au/def/Method/VOL> a skos:Concept ;
    rdfs:isDefinedBy cs: ;
    skos:altLabel "VOL"@en ;
    skos:definition "Volumetric or titrimetric analyses are quantitative analytical techniques which employ a titration in comparing an unknown with a standard.  In a titration, a volume of a standardized solution contain"@en ;
    skos:inScheme cs: ;
    skos:prefLabel "Volumetric"@en ;
    skos:scopeNote "Volumetric or titrimetric analyses are quantitative analytical techniques which employ a titration in comparing an unknown with a standard.  In a titration, a volume of a standardized solution containing a known concentration of reactant \"A\" is added incrementally to a sample containing an unknown concentration of reactant \"B\".  The titration proceeds until reactant \"B\" is just consumed (stoichiometric completion).  This is known as the equivalence point.  At this point the number of equivalents of \"A\" added to the unknown equals the number of equivalents of \"B\" originally present in the unknown.  Volumetric methods have the potential for a precision of up to 0.1%. http://www.ecs.umass.edu/cee/reckhow/courses/572/572bk16/572BK16.html"@en ;
    skos:topConceptOf cs: .

<http://pid.geoscience.gov.au/def/Method/Visual> a skos:Concept ;
    rdfs:isDefinedBy cs: ;
    skos:altLabel "Visual"@en ;
    skos:definition "an observation has been made by eye and a subjective evaluation has been made."@en ;
    skos:inScheme cs: ;
    skos:prefLabel "Visual"@en ;
    skos:topConceptOf cs: .

<http://pid.geoscience.gov.au/def/Method/WHOLE_OIL_GC> a skos:Concept ;
    rdfs:isDefinedBy cs: ;
    skos:altLabel "WHOLE_OIL_GC"@en ;
    skos:definition "\"Whole Oil Gas Chromatography: a mixture is separated by distributing the components between a stationary phase and a mobile phase. The stationary phase is a high-boiling liquid. This high-boiliing li"@en ;
    skos:inScheme cs: ;
    skos:prefLabel "Whole Oil Gas Chromatography"@en ;
    skos:scopeNote "\"Whole Oil Gas Chromatography: a mixture is separated by distributing the components between a stationary phase and a mobile phase. The stationary phase is a high-boiling liquid. This high-boiliing liquid is packed into a long, narrow glass or metal column. The mixture to be analyzed is loaded by syringe into the beginning of this column. The mobile phase is an inert gas which continuously flows through the column. The components of the mixture distribute between the stationary high-boiling liquid (these components are either condensed or absorbed on the high-boiling liquid) and mobile gas (vapor) phase moving through the column. The gaseous mixture flows through a detector at the end of the column and if it has been successfully separated, the components show as different peaks on a recorder. http://orgchem.colorado.edu/hndbksupport/chrom.html\""@en ;
    skos:topConceptOf cs: .

<http://pid.geoscience.gov.au/def/Method/WQ_Sonde> a skos:Concept ;
    rdfs:isDefinedBy cs: ;
    skos:altLabel "WQ Sonde"@en ;
    skos:definition "Multiparameter sensor instrument used for sampling, monitoring and logging data in surface water applications, ranging from ponds to rivers to estuaries (e.g. YSI probe)"@en ;
    skos:inScheme cs: ;
    skos:prefLabel "Water Quality Sonde"@en ;
    skos:topConceptOf cs: .

<http://pid.geoscience.gov.au/def/Method/XRD> a skos:Concept ;
    rdfs:isDefinedBy cs: ;
    skos:altLabel "XRD"@en ;
    skos:definition "XRD: X-ray Diffraction. A non-destructive technique in which a beam of X-rays is foccussed on a powdered sample where crystals have varied and random orientation. The patterns are compared with refere"@en ;
    skos:inScheme cs: ;
    skos:prefLabel "X-Ray Diffraction"@en ;
    skos:scopeNote "XRD: X-ray Diffraction. A non-destructive technique in which a beam of X-rays is foccussed on a powdered sample where crystals have varied and random orientation. The patterns are compared with reference standards to identify the minerals present. "@en ;
    skos:topConceptOf cs: .

<http://pid.geoscience.gov.au/def/Method/XRF> a skos:Concept ;
    rdfs:isDefinedBy cs: ;
    skos:altLabel "XRF"@en ;
    skos:definition "XRF: A non-destructive technique that can be used to quantify elemental constituents of solid and liquid samples. XRF measures the intensity of emitted radiation, from a fused glass or pressed powder "@en ;
    skos:inScheme cs: ;
    skos:prefLabel "X-ray Fluorescence"@en ;
    skos:scopeNote "XRF: A non-destructive technique that can be used to quantify elemental constituents of solid and liquid samples. XRF measures the intensity of emitted radiation, from a fused glass or pressed powder sample.  XRF is  one of the best analytical tools for determination of major and trace elements in samples. Detection limits can be as good as 0.2 ppm, more commonly about 1 - 3 ppm."@en ;
    skos:topConceptOf cs: .

<http://pid.geoscience.gov.au/def/Method/micro-Kjeldahl> a skos:Concept ;
    rdfs:isDefinedBy cs: ;
    skos:altLabel "micro-Kjeldahl"@en ;
    skos:definition "Method for the determination of nitrogen in organic and in-organic substances. The method can be broken down in three main steps; digestion, distilliantion and titration. The amount of nitrogen in a s"@en ;
    skos:inScheme cs: ;
    skos:prefLabel "micro-Kjeldahl"@en ;
    skos:scopeNote "Method for the determination of nitrogen in organic and in-organic substances. The method can be broken down in three main steps; digestion, distilliantion and titration. The amount of nitrogen in a sample can be calculated from the quantified amount of ammonia ions in the receiving solution. http://www.labconco.com/pdf/kjeldahl/guide_kjeldahl.pdf"@en ;
    skos:topConceptOf cs: .

<http://pid.geoscience.gov.au/def/Method/pipette> a skos:Concept ;
    rdfs:isDefinedBy cs: ;
    skos:altLabel "pipette"@en ;
    skos:definition "The grain-size distribution of muddy sediments (silt and clay sizes) is commonly determined by pipette analysis. The sample is placed in a one-liter graduated cylinder filled with distilled water and "@en ;
    skos:inScheme cs: ;
    skos:prefLabel "pipette analysis"@en ;
    skos:scopeNote "The grain-size distribution of muddy sediments (silt and clay sizes) is commonly determined by pipette analysis. The sample is placed in a one-liter graduated cylinder filled with distilled water and a dispersing agent to prevent clay flocculation. http://geology.uprm.edu/Morelock/character.htm"@en ;
    skos:topConceptOf cs: .

<https://linked.data.gov.au/org/ga/voc-wg> a sdo:Organization ;
    sdo:affiliation <https://linked.data.gov.au/org/ga> ;
    sdo:name "Geoscience Australia Vocabulary Working Group" ;
    sdo:url <https://www.ga.gov.au/data-pubs/datastandards> .

<https://linked.data.gov.au/org/ga> a sdo:Organization ;
    sdo:name "Geoscience Australia" ;
    sdo:url <https://www.ga.gov.au> .

cs: a skos:ConceptScheme ;
    dcterms:created "2019-03-12T11:48:09"^^xsd:dateTime ;
    dcterms:creator <https://linked.data.gov.au/org/ga/voc-wg> ;
    dcterms:modified "2019-03-12T11:48:09"^^xsd:dateTime ;
    dcterms:provenance "GA's ORAPROD database tables"@en ;
    dcterms:publisher <https://linked.data.gov.au/org/ga> ;
    skos:changeNote "This vocabulary created directly from the database"@en ;
    skos:definition "Geoscience Australia's 12-Mar-2019 version of the Method vocabulary"@en ;
    skos:hasTopConcept <http://pid.geoscience.gov.au/def/Method/AAS>,
        <http://pid.geoscience.gov.au/def/Method/AC>,
        <http://pid.geoscience.gov.au/def/Method/ADCP>,
        <http://pid.geoscience.gov.au/def/Method/AMS>,
        <http://pid.geoscience.gov.au/def/Method/APM>,
        <http://pid.geoscience.gov.au/def/Method/Ar_Ar>,
        <http://pid.geoscience.gov.au/def/Method/BULK>,
        <http://pid.geoscience.gov.au/def/Method/Bomb>,
        <http://pid.geoscience.gov.au/def/Method/CLSM>,
        <http://pid.geoscience.gov.au/def/Method/COL>,
        <http://pid.geoscience.gov.au/def/Method/CSIA_GAS>,
        <http://pid.geoscience.gov.au/def/Method/CSIA_OIL>,
        <http://pid.geoscience.gov.au/def/Method/Calculate>,
        <http://pid.geoscience.gov.au/def/Method/Chaix_Meca>,
        <http://pid.geoscience.gov.au/def/Method/Chart_depth>,
        <http://pid.geoscience.gov.au/def/Method/DIC>,
        <http://pid.geoscience.gov.au/def/Method/Derivation>,
        <http://pid.geoscience.gov.au/def/Method/Digestion>,
        <http://pid.geoscience.gov.au/def/Method/ELEMENTS>,
        <http://pid.geoscience.gov.au/def/Method/EM>,
        <http://pid.geoscience.gov.au/def/Method/EOM>,
        <http://pid.geoscience.gov.au/def/Method/EOS>,
        <http://pid.geoscience.gov.au/def/Method/ESR>,
        <http://pid.geoscience.gov.au/def/Method/Echo>,
        <http://pid.geoscience.gov.au/def/Method/FILA>,
        <http://pid.geoscience.gov.au/def/Method/Fluorometry>,
        <http://pid.geoscience.gov.au/def/Method/GAS>,
        <http://pid.geoscience.gov.au/def/Method/GC>,
        <http://pid.geoscience.gov.au/def/Method/GCMS_ARO_FS>,
        <http://pid.geoscience.gov.au/def/Method/GCMS_ARO_MRM>,
        <http://pid.geoscience.gov.au/def/Method/GCMS_ARO_SIR>,
        <http://pid.geoscience.gov.au/def/Method/GCMS_SAT_FS>,
        <http://pid.geoscience.gov.au/def/Method/GCMS_SAT_MRM>,
        <http://pid.geoscience.gov.au/def/Method/GCMS_SAT_SIR>,
        <http://pid.geoscience.gov.au/def/Method/GRS>,
        <http://pid.geoscience.gov.au/def/Method/Gravimetry>,
        <http://pid.geoscience.gov.au/def/Method/H20>,
        <http://pid.geoscience.gov.au/def/Method/ICA>,
        <http://pid.geoscience.gov.au/def/Method/ICP-MS>,
        <http://pid.geoscience.gov.au/def/Method/ICP-OES>,
        <http://pid.geoscience.gov.au/def/Method/INAA>,
        <http://pid.geoscience.gov.au/def/Method/IRMS>,
        <http://pid.geoscience.gov.au/def/Method/ISOTOPES>,
        <http://pid.geoscience.gov.au/def/Method/ISOTOPES_IN>,
        <http://pid.geoscience.gov.au/def/Method/KINETICS>,
        <http://pid.geoscience.gov.au/def/Method/K_Ar>,
        <http://pid.geoscience.gov.au/def/Method/LA-ICP-MS>,
        <http://pid.geoscience.gov.au/def/Method/LECO>,
        <http://pid.geoscience.gov.au/def/Method/LRMP>,
        <http://pid.geoscience.gov.au/def/Method/Laser>,
        <http://pid.geoscience.gov.au/def/Method/Leica_1350>,
        <http://pid.geoscience.gov.au/def/Method/Lk-MDS600>,
        <http://pid.geoscience.gov.au/def/Method/Lk-THM600>,
        <http://pid.geoscience.gov.au/def/Method/Lk-TS1500>,
        <http://pid.geoscience.gov.au/def/Method/MF>,
        <http://pid.geoscience.gov.au/def/Method/MIMS>,
        <http://pid.geoscience.gov.au/def/Method/MPIP>,
        <http://pid.geoscience.gov.au/def/Method/MacFlinCor>,
        <http://pid.geoscience.gov.au/def/Method/Microscopy>,
        <http://pid.geoscience.gov.au/def/Method/NMM>,
        <http://pid.geoscience.gov.au/def/Method/OIL_FRACTION>,
        <http://pid.geoscience.gov.au/def/Method/PIXE>,
        <http://pid.geoscience.gov.au/def/Method/PY_GC>,
        <http://pid.geoscience.gov.au/def/Method/REFLECTANCE>,
        <http://pid.geoscience.gov.au/def/Method/ROCKEVAL>,
        <http://pid.geoscience.gov.au/def/Method/Rb_Sr>,
        <http://pid.geoscience.gov.au/def/Method/Rock-colour_Chart>,
        <http://pid.geoscience.gov.au/def/Method/SAA>,
        <http://pid.geoscience.gov.au/def/Method/SEMCL>,
        <http://pid.geoscience.gov.au/def/Method/SHRIMP>,
        <http://pid.geoscience.gov.au/def/Method/STM>,
        <http://pid.geoscience.gov.au/def/Method/SYNCXRF>,
        <http://pid.geoscience.gov.au/def/Method/Settling_Tube>,
        <http://pid.geoscience.gov.au/def/Method/Sieve>,
        <http://pid.geoscience.gov.au/def/Method/Sm_Nd>,
        <http://pid.geoscience.gov.au/def/Method/Sync-FTIR>,
        <http://pid.geoscience.gov.au/def/Method/TIT>,
        <http://pid.geoscience.gov.au/def/Method/Transmissometry_>,
        <http://pid.geoscience.gov.au/def/Method/Turbidimetry>,
        <http://pid.geoscience.gov.au/def/Method/USGS_H_F>,
        <http://pid.geoscience.gov.au/def/Method/UV_VIS>,
        <http://pid.geoscience.gov.au/def/Method/U_Pb_Conventional>,
        <http://pid.geoscience.gov.au/def/Method/Unknown>,
        <http://pid.geoscience.gov.au/def/Method/VGT>,
        <http://pid.geoscience.gov.au/def/Method/VOL>,
        <http://pid.geoscience.gov.au/def/Method/Visual>,
        <http://pid.geoscience.gov.au/def/Method/WHOLE_OIL_GC>,
        <http://pid.geoscience.gov.au/def/Method/WQ_Sonde>,
        <http://pid.geoscience.gov.au/def/Method/XRD>,
        <http://pid.geoscience.gov.au/def/Method/XRF>,
        <http://pid.geoscience.gov.au/def/Method/micro-Kjeldahl>,
        <http://pid.geoscience.gov.au/def/Method/pipette> ;
    skos:prefLabel "Method"@en .

