PREFIX : <https://pid.geoscience.gov.au/def/voc/ga/GeomorphologyGeneral/>
PREFIX cs: <https://pid.geoscience.gov.au/def/voc/ga/GeomorphologyGeneral>
PREFIX dcat: <http://www.w3.org/ns/dcat#>
PREFIX isoroles: <https://linked.data.gov.au/def/data-roles/>
PREFIX owl: <http://www.w3.org/2002/07/owl#>
PREFIX prov: <http://www.w3.org/ns/prov#>
PREFIX rdfs: <http://www.w3.org/2000/01/rdf-schema#>
PREFIX schema: <https://schema.org/>
PREFIX skos: <http://www.w3.org/2004/02/skos/core#>
PREFIX xsd: <http://www.w3.org/2001/XMLSchema#>

:BGU-Type
    a skos:Concept ;
    rdfs:isDefinedBy cs: ;
    skos:altLabel "BGU-T"@en ;
    skos:definition "BGU-T are defined for commonly used sub-categories of BGU, and can always be simplified up to their BGU and SETTING/PROCESS categories (Nanson et al., 2023)."@en ;
    skos:inScheme cs: ;
    skos:prefLabel "BGU - Type"@en ;
    skos:topConceptOf cs: ;
.

<https://pid.geoscience.gov.au/def/voc/ga/GeomorphologyGeneral/BGU–sub-type>
    a skos:Concept ;
    rdfs:isDefinedBy cs: ;
    skos:altLabel "BGU-sT"@en ;
    skos:definition "BGU-sT provide more granular classification of BGU-T, but can always be simplified up to their BGU-T, BGU and SETTING/PROCESS categories (Nanson et al., 2023). BGU-sT definitions are not included in this glossary."@en ;
    skos:inScheme cs: ;
    skos:prefLabel "BGU – sub-Type"@en ;
    skos:topConceptOf cs: ;
.

:abyssal_plain
    a skos:Concept ;
    rdfs:isDefinedBy cs: ;
    skos:definition "An extensive, flat or gently sloping region, usually found at depths greater than 4 km, covered by up to 1 km sediment thicknesses consisting of fine-grained erosional detritus and biogenic particles (Harff et al., 2016)."@en ;
    skos:inScheme cs: ;
    skos:prefLabel "abyssal plain"@en ;
    skos:topConceptOf cs: ;
.

:accretionary_prism
    a skos:Concept ;
    rdfs:isDefinedBy cs: ;
    skos:definition "Sedimentary wedge at a convergent plate margin above a subduction zone created by material of the subducting lower plate scraped off and transferred to the overriding upper plate (modified after Harff et al., 2016)."@en ;
    skos:inScheme cs: ;
    skos:prefLabel "accretionary prism"@en ;
    skos:topConceptOf cs: ;
.

:age_relative_modern
    a skos:Concept ;
    rdfs:isDefinedBy cs: ;
    skos:definition "Units formed by active processes, typically more recently than the Late Holocene"@en ;
    skos:inScheme cs: ;
    skos:prefLabel "age, relative: modern"@en ;
    skos:topConceptOf cs: ;
.

:age_relative_palimpsest
    a skos:Concept ;
    rdfs:isDefinedBy cs: ;
    skos:definition "Units that are relict in origin but which are still undergoing modification by modern processes."@en ;
    skos:inScheme cs: ;
    skos:prefLabel "age, relative: palimpsest"@en ;
    skos:topConceptOf cs: ;
.

:age_relative_relict
    a skos:Concept ;
    rdfs:isDefinedBy cs: ;
    skos:definition "Units that formed prior to the Late Holocene under a different process regime to the present, and which are no longer active."@en ;
    skos:inScheme cs: ;
    skos:prefLabel "age, relative: relict"@en ;
    skos:topConceptOf cs: ;
.

:axial_high
    a skos:Concept ;
    rdfs:isDefinedBy cs: ;
    skos:definition "Elongated ridge up to 15–20 km wide and 500 m high relative to nearby abyssal plain with the shallowest points around neovolcanic zone. The presence of axial highs is due to the upwelling of hot mantle beneath fast spreading centres (Harff et al., 2016)."@en ;
    skos:inScheme cs: ;
    skos:prefLabel "axial high"@en ;
    skos:topConceptOf cs: ;
.

:axial_valley
    a skos:Concept ;
    rdfs:isDefinedBy cs: ;
    skos:definition "The axial depression of a MID-OCEAN RIDGE, characteristic of slow spreading centers (Harff et al., 2016)"@en ;
    skos:inScheme cs: ;
    skos:prefLabel "axial valley"@en ;
    skos:topConceptOf cs: ;
.

:back-arc_basin
    a skos:Concept ;
    rdfs:isDefinedBy cs: ;
    skos:definition "An oceanic basin behind a volcanic arc associated with an intraoceanic subduction zone (modified after Harff et al., 2016)."@en ;
    skos:inScheme cs: ;
    skos:prefLabel "back-arc basin"@en ;
    skos:topConceptOf cs: ;
.

:basic_geomorphic_unit
    a skos:Concept ;
    rdfs:isDefinedBy cs: ;
    skos:altLabel "BGU"@en ;
    skos:definition """BGU are the broadest geomorphic terms used to classify Part 1 (MORPHOLOGY) FEATURE 
shapes and can always be simplified up to their SETTING/PROCESS categories (Nanson et al., 2023)."""@en ;
    skos:inScheme cs: ;
    skos:prefLabel "Basic Geomorphic Unit"@en ;
    skos:topConceptOf cs: ;
.

:continental_rise
    a skos:Concept ;
    rdfs:isDefinedBy cs: ;
    skos:definition "A gentle slope rising from the oceanic depths towards the foot of a CONTINENTAL SLOPE, created by the accumulation of sediments at the foot of CONTINENTAL SLOPES (Harris et al., 2014)."@en ;
    skos:inScheme cs: ;
    skos:prefLabel "continental rise"@en ;
    skos:topConceptOf cs: ;
.

:continental_shelf
    a skos:Concept ;
    rdfs:isDefinedBy cs: ;
    skos:definition "The seabed regionadjacent to a continent (or around an island), composed of continental crust, and extending from the low-water line to a depth at which there is usually a marked increase of slope towards oceanic depths (modified after Harris et al., 2014)."@en ;
    skos:inScheme cs: ;
    skos:prefLabel "continental shelf"@en ;
    skos:topConceptOf cs: ;
.

:continental_slope
    a skos:Concept ;
    rdfs:isDefinedBy cs: ;
    skos:definition "Geological boundary marking the transition between continental and oceanic crust. It is located seaward from the shelf edge to the upper edge of a CONTINENTAL RISE or the point where there is a general reduction in slope. There are two kinds of CONTINENTAL SLOPE, one associated with passive continental margins, the other with active margins (Harff et al., 2016)"@en ;
    skos:inScheme cs: ;
    skos:prefLabel "continental slope"@en ;
    skos:topConceptOf cs: ;
.

:depth_relative_buried
    a skos:Concept ;
    rdfs:isDefinedBy cs: ;
    skos:definition "Units that have been mapped either at the surface or in the sub-surface (e.g. using sub-bottom imagery) and have minimal surface expression (e.g. a buried FLUVIAL VALLEY visible in sub-bottom data)."@en ;
    skos:inScheme cs: ;
    skos:prefLabel "depth, relative: buried"@en ;
    skos:topConceptOf cs: ;
.

:depth_relative_partially-buried
    a skos:Concept ;
    rdfs:isDefinedBy cs: ;
    skos:definition "Geomorphic units that have clear, though partial, seafloor expression (e.g. coarser-grained BEDFORMS amongst muddier PLANE BED)."@en ;
    skos:inScheme cs: ;
    skos:prefLabel "depth, relative: partially-buried"@en ;
    skos:topConceptOf cs: ;
.

:depth_relative_surface
    a skos:Concept ;
    rdfs:isDefinedBy cs: ;
    skos:definition "Units that have been mapped at the surface and have minimal discernible buried component"@en ;
    skos:inScheme cs: ;
    skos:prefLabel "depth, relative: surface"@en ;
    skos:topConceptOf cs: ;
.

:feature
    a skos:Concept ;
    rdfs:isDefinedBy cs: ;
    skos:definition """A list of terms that are used to define seafloor MORPHOLOGY; these were primarily sourced 
from the list of terms and definitions provided in the IHO (International Hydrographic 
Organization, 2019) list of undersea Feature Names which were subsequently updated and 
illustrated in Dove et al., (2020: Part 1). MORPHOLOGY FEATURE terms (e.g. Ridge, Canyon) are capitalised as proper nouns to help distinguish them from more general morphological 
descriptors (e.g. upper canyon, canyon wall, crests; Dove et al., 2020)"""@en ;
    skos:inScheme cs: ;
    skos:prefLabel "Feature"@en ;
    skos:topConceptOf cs: ;
.

:field_of_units
    a skos:Concept ;
    rdfs:isDefinedBy cs: ;
    skos:definition "Delineation of groups of smaller geomorphic units that may or may not be individually and / or partially mapped (e.g. a polygon defining a field of partially mapped DUNES; a polygon defining a field of submarine GULLIES)"@en ;
    skos:inScheme cs: ;
    skos:prefLabel "Field (of units)"@en ;
    skos:topConceptOf cs: ;
.

:fore-arc_basin
    a skos:Concept ;
    rdfs:isDefinedBy cs: ;
    skos:definition "An oceanic basin in forearc regions between the OCEANIC TRENCH and the volcanic front (modified after Harff et al., 2016)."@en ;
    skos:inScheme cs: ;
    skos:prefLabel "fore-arc basin"@en ;
    skos:topConceptOf cs: ;
.

:geomorphology
    a skos:Concept ;
    rdfs:isDefinedBy cs: ;
    skos:definition "The study of the shape of the Earth's surface and the processes forming them (modified from Harris and Baker, 2011). This may include, but is distinct from, geomorphometry - the science of quantitative terrain characterisation, which encompasses acquisition and processing of topographic data as well as analyses and applications related to geomorphology (see Lecours et al., 2016). “Marine Geomorphology” is used in specific reference to Part 2 GEOMORPHOLOGY (Nanson et al., 2023) and the UNITS defined therein."@en ;
    skos:inScheme cs: ;
    skos:prefLabel "Geomorphology"@en ;
    skos:topConceptOf cs: ;
.

:grain-size_texture
    a skos:Concept ;
    rdfs:isDefinedBy cs: ;
    skos:definition "The proportion of mud, sand and gravel that comprise a sample, described using the Folk (1954) classification scheme."@en ;
    skos:inScheme cs: ;
    skos:prefLabel "grain size: texture"@en ;
    skos:topConceptOf cs: ;
.

:grain_size_particle_size
    a skos:Concept ;
    rdfs:isDefinedBy cs: ;
    skos:definition "The size distribution of a unit sample, described using the Wentworth (1922) scheme."@en ;
    skos:inScheme cs: ;
    skos:prefLabel "grain size: particle size"@en ;
    skos:topConceptOf cs: ;
.

:island_arc
    a skos:Concept ;
    rdfs:isDefinedBy cs: ;
    skos:definition "Marine subset of currently active or formerly active VOLCANOES located near the boundary between two converging tectonic plates. The VOLCANOES are located 150–350 km away from the OCEANIC TRENCH on the overlying plate and define an arc in plan view (modified after Harff et al., 2016)."@en ;
    skos:inScheme cs: ;
    skos:prefLabel "island arc"@en ;
    skos:topConceptOf cs: ;
.

:landform
    a skos:Concept ;
    rdfs:isDefinedBy cs: ;
    skos:definition "One of the central study objects in the field of geomorphology (the other objects being special linear or point features, like break lines, thalwegs or peaks), a feature of the land surface with conspicuous shape and distinct characteristics (Evans, 2012; MacMillan and Shary, 2009)"@en ;
    skos:inScheme cs: ;
    skos:prefLabel "Landform"@en ;
    skos:topConceptOf cs: ;
.

:lithology
    a skos:Concept ;
    rdfs:isDefinedBy cs: ;
    skos:definition "Categories for defining the composition of geomorphic units may include, but are not limited to: siliclastic, carbonate, beach rock or bedrock"@en ;
    skos:inScheme cs: ;
    skos:prefLabel "lithology"@en ;
    skos:topConceptOf cs: ;
.

:marginal_marine_process
    a skos:Concept ;
    rdfs:isDefinedBy cs: ;
    skos:definition "The relative contribution of wave, tide and fluvial processes that have formed a unit. E.g. A mapped MOUTHBAR may be fluvial-dominated, tide-influenced and wave-affected (Ftw Ainsworth et al., 2011)."@en ;
    skos:inScheme cs: ;
    skos:prefLabel "marginal marine process"@en ;
    skos:topConceptOf cs: ;
.

:mid-ocean_ridge
    a skos:Concept ;
    rdfs:isDefinedBy cs: ;
    skos:definition "A linear, narrow volcanic and tectonic region which marks the constructive boundary between two tectonic plates. It is divided into segments by transform FAULTS and other offsets. Depending on the speed of the spreading centre, AXIAL HIGHS or AXIAL VALLEYS can form (Harff et al., 2016)"@en ;
    skos:inScheme cs: ;
    skos:prefLabel "mid-ocean ridge"@en ;
    skos:topConceptOf cs: ;
.

:morphology
    a skos:Concept ;
    rdfs:isDefinedBy cs: ;
    skos:definition """The shape of the seafloor surface. Where capitalised, “Morphology” is used in specific 
reference to Part 1 MORPHOLOGY (Dove et al., 2020) and the FEATURES defined therein"""@en ;
    skos:inScheme cs: ;
    skos:prefLabel "Morphology"@en ;
    skos:topConceptOf cs: ;
.

:morphometrics
    a skos:Concept ;
    rdfs:isDefinedBy cs: ;
    skos:definition """Quantitative analysis of the external shape and size of morphological features. Terrain 
derivatives such as: bathymetric position index (BPI), terrain ruggedness index, slope, aspect, curvature and rugosity are widely used as morphometric parameters with the help of geographic information systems."""@en ;
    skos:inScheme cs: ;
    skos:prefLabel "morphometrics"@en ;
    skos:topConceptOf cs: ;
.

:oceanic_trench
    a skos:Concept ;
    rdfs:isDefinedBy cs: ;
    skos:definition "Elongated, deep and narrow trench between the ABYSSAL PLAINS and the border of the upper plate where oceanic lithosphere is bent downward under the margin of the upper plate and dives into the asthenosphere. An oceanic trench is about 2 km deeper than the surrounding ocean floor (Harff et al., 2016)."@en ;
    skos:inScheme cs: ;
    skos:prefLabel "oceanic trench"@en ;
    skos:topConceptOf cs: ;
.

:physiography
    a skos:Concept ;
    rdfs:isDefinedBy cs: ;
    skos:definition "Terms that are used to describe the macroscale physical expression of the seafloor (e.g. CONTINENTAL SHELF). Physiographic terms were primarily derived from Harris et al (2014) global seafloor geomorphology map, however, their complete list of terms have been split between PHYSIOGRAPHIC, Part 1 (MORPHOLOGY) and Part 2 (GEOMORPHOLOGY) vocabularies."@en ;
    skos:inScheme cs: ;
    skos:prefLabel "Physiography"@en ;
    skos:topConceptOf cs: ;
.

:process
    a skos:Concept ;
    rdfs:isDefinedBy cs: ;
    skos:definition """The term PROCESS is used herein to group geomorphic units formed by similar processes and 
are the broadest (alongside SETTING) Part 2 terms for classifying Part 1 Morphology FEATURES."""@en ;
    skos:inScheme cs: ;
    skos:prefLabel "Process"@en ;
    skos:topConceptOf cs: ;
.

:sea_level_regressive
    a skos:Concept ;
    rdfs:isDefinedBy cs: ;
    skos:definition "Units formed during a shoreline regression (seaward advance) associated with a relative sea-level fall (forced or normal; (Muto and Steel, 1997)"@en ;
    skos:inScheme cs: ;
    skos:prefLabel "sea level: regressive"@en ;
    skos:topConceptOf cs: ;
.

:sea_level_stillstand
    a skos:Concept ;
    rdfs:isDefinedBy cs: ;
    skos:definition "Units formed during a relative sea-level stillstand (Muto and Steel, 1997)"@en ;
    skos:inScheme cs: ;
    skos:prefLabel "sea level: stillstand"@en ;
    skos:topConceptOf cs: ;
.

:sea_level_transgressive
    a skos:Concept ;
    rdfs:isDefinedBy cs: ;
    skos:definition "Units formed during a shoreline transgression (landward migration) associated with a relative sea-level rise (Muto and Steel, 1997)"@en ;
    skos:inScheme cs: ;
    skos:prefLabel "sea level: transgressive"@en ;
    skos:topConceptOf cs: ;
.

:setting
    a skos:Concept ;
    rdfs:isDefinedBy cs: ;
    skos:definition """Used herein, the term SETTING is used to group geomorphic units formed in specific 
environments and are the broadest (alongside PROCESS) Part 2 terms for classifying Part 1 
Morphology FEATURES."""@en ;
    skos:inScheme cs: ;
    skos:prefLabel "Setting"@en ;
    skos:topConceptOf cs: ;
.

:unit
    a skos:Concept ;
    rdfs:isDefinedBy cs: ;
    skos:definition "Used herein, the term UNIT refers to a three-dimensional geomorphic interpretation of (Part1: MORPHOLOGY) FEATURES, and usually incorporate both sub-surface (stratigraphic) and formative process interpretations."@en ;
    skos:inScheme cs: ;
    skos:prefLabel "Unit"@en ;
    skos:topConceptOf cs: ;
.

cs:
    a skos:ConceptScheme ;
    owl:versionIRI :1.0 ;
    skos:definition """A vocabulary of general terms used to support the application of the two-part seabed geomorphology classification scheme. This vocabulary is the product of a collaboration between marine geoscientists from marine mapping programmes/networks in Norway (MAREANO), Ireland (INFOMAR), UK (MAREMAP), and Australia (Geoscience Australia). 
Definitions in this vocabulary are subject to intermittent review and versioning. """@en ;
    skos:hasTopConcept
        :BGU-Type ,
        <https://pid.geoscience.gov.au/def/voc/ga/GeomorphologyGeneral/BGU–sub-type> ,
        :abyssal_plain ,
        :accretionary_prism ,
        :age_relative_modern ,
        :age_relative_palimpsest ,
        :age_relative_relict ,
        :axial_high ,
        :axial_valley ,
        :back-arc_basin ,
        :basic_geomorphic_unit ,
        :continental_rise ,
        :continental_shelf ,
        :continental_slope ,
        :depth_relative_buried ,
        :depth_relative_partially-buried ,
        :depth_relative_surface ,
        :feature ,
        :field_of_units ,
        :fore-arc_basin ,
        :geomorphology ,
        :grain-size_texture ,
        :grain_size_particle_size ,
        :island_arc ,
        :landform ,
        :lithology ,
        :marginal_marine_process ,
        :mid-ocean_ridge ,
        :morphology ,
        :morphometrics ,
        :oceanic_trench ,
        :physiography ,
        :process ,
        :sea_level_regressive ,
        :sea_level_stillstand ,
        :sea_level_transgressive ,
        :setting ,
        :unit ;
    skos:historyNote "This vocabulary describes the glossary in Part 2 of the two-part seabed geomorphology classification scheme DOI: 10.5281/zenodo.7804019"@en ;
    skos:prefLabel "Marine Geomorphology - Method Terms and Physiography"@en ;
    prov:qualifiedAttribution
        [
            dcat:hadRole isoroles:custodian ;
            prov:agent
                [
                    a schema:Person ;
                    schema:email ""^^xsd:anyURI ;
                    schema:name "Poc: Rachel Nanson" ;
                ] ;
        ] ,
        [
            dcat:hadRole isoroles:custodian ;
            prov:agent
                [
                    a schema:Person ;
                    schema:email ""^^xsd:anyURI ;
                    schema:name "Marine And Coastal Geoscience" ;
                ] ;
        ] ,
        [
            dcat:hadRole isoroles:custodian ;
            prov:agent
                [
                    a schema:Person ;
                    schema:email ""^^xsd:anyURI ;
                    schema:name "Orca Branch" ;
                ] ;
        ] ;
    schema:creator
        [
            a schema:Organization ;
            schema:name "Ga" ;
            schema:url ""^^xsd:anyURI ;
        ] ;
    schema:dateCreated "2024-05-22"^^xsd:date ;
    schema:dateModified "2024-05-22"^^xsd:date ;
    schema:publisher
        [
            a schema:Organization ;
            schema:name "Ga" ;
            schema:url ""^^xsd:anyURI ;
        ] ;
    schema:version "1.0" ;
.
