PREFIX : <https://pid.geoscience.gov.au/def/voc/ga/WasteStorageType/>
PREFIX cs: <https://pid.geoscience.gov.au/def/voc/ga/WasteStorageType>
PREFIX dcat: <http://www.w3.org/ns/dcat#>
PREFIX isoroles: <https://linked.data.gov.au/def/data-roles/>
PREFIX owl: <http://www.w3.org/2002/07/owl#>
PREFIX prov: <http://www.w3.org/ns/prov#>
PREFIX rdfs: <http://www.w3.org/2000/01/rdf-schema#>
PREFIX schema: <https://schema.org/>
PREFIX skos: <http://www.w3.org/2004/02/skos/core#>
PREFIX xsd: <http://www.w3.org/2001/XMLSchema#>

:surface
    a skos:Concept ;
    rdfs:isDefinedBy cs: ;
    skos:definition "Uncovered mining waste storage."@en ;
    skos:inScheme cs: ;
    skos:prefLabel "surface"@en ;
    skos:topConceptOf cs: ;
    schema:citation "http://resource.geosciml.org/classifier/cgi/waste-storage/surface"^^xsd:anyURI ;
.

:underground
    a skos:Concept ;
    rdfs:isDefinedBy cs: ;
    skos:definition "Mining waste storage in an underground environment."@en ;
    skos:inScheme cs: ;
    skos:prefLabel "underground"@en ;
    skos:topConceptOf cs: ;
    schema:citation "http://resource.geosciml.org/classifier/cgi/waste-storage/underground"^^xsd:anyURI ;
.

:underwater
    a skos:Concept ;
    rdfs:isDefinedBy cs: ;
    skos:definition "Mining waste storage below a natural water body."@en ;
    skos:inScheme cs: ;
    skos:prefLabel "underwater"@en ;
    skos:topConceptOf cs: ;
    schema:citation "http://resource.geosciml.org/classifier/cgi/waste-storage/underwater"^^xsd:anyURI ;
.

:water_cover
    a skos:Concept ;
    rdfs:isDefinedBy cs: ;
    skos:broader :covered ;
    skos:definition "Mining waste covered by an engineered water body - (e.g. engineered tailing storage facility (TSF) with a water cover, in-pit tailings with a water cover)."@en ;
    skos:inScheme cs: ;
    skos:prefLabel "water cover"@en ;
.

:covered
    a skos:Concept ;
    rdfs:isDefinedBy cs: ;
    skos:definition "Covered mining waste storage, with covers typically comprising soil, rock, geosynthetics, plastics or other materials."@en ;
    skos:inScheme cs: ;
    skos:narrower :water_cover ;
    skos:prefLabel "covered"@en ;
    skos:topConceptOf cs: ;
    schema:citation "http://resource.geosciml.org/classifier/cgi/waste-storage/covered"^^xsd:anyURI ;
.

cs:
    a skos:ConceptScheme ;
    owl:versionIRI :1.0 ;
    skos:definition "Terms used in the Geoscience Australia Commodities database that describe the storage type a mining waste feature may have."@en ;
    skos:hasTopConcept
        :covered ,
        :surface ,
        :underground ,
        :underwater ;
    skos:historyNote "Geoscience Australia Commodities (OZMIN.LU_STORAGE_TYPE)"@en ;
    skos:prefLabel "Mineral Resources (OZMIN) - Waste Storage Types"@en ;
    prov:qualifiedAttribution
        [
            dcat:hadRole isoroles:custodian ;
            prov:agent
                [
                    a schema:Person ;
                    schema:email ""^^xsd:anyURI ;
                    schema:name "Team Lead   Information Services. Minerals" ;
                ] ;
        ] ,
        [
            dcat:hadRole isoroles:custodian ;
            prov:agent
                [
                    a schema:Person ;
                    schema:email ""^^xsd:anyURI ;
                    schema:name "Energy And Groundwater Division." ;
                ] ;
        ] ;
    schema:creator
        [
            a schema:Organization ;
            schema:name "Ga" ;
            schema:url ""^^xsd:anyURI ;
        ] ;
    schema:dateCreated "2022-04-13"^^xsd:date ;
    schema:dateModified "2024-02-22"^^xsd:date ;
    schema:publisher
        [
            a schema:Organization ;
            schema:name "Ga" ;
            schema:url ""^^xsd:anyURI ;
        ] ;
    schema:version "1.0" ;
.
